src/RqRsInvDownLock.v
@@ -1,0 +1,482 @@
+Require Import Peano_dec Omega List ListSupport.
+Require Import Common FMap.
+Require Import Syntax Semantics SemFacts StepM Invariant Serial.
+Require Import Reduction Commutativity QuasiSeq Topology.
+Require Import RqRsTopo RqRsFacts RqRsInvMsg.
+
+Set Implicit Arguments.
+
+Open Scope list.
+Open Scope fmap.
+
+Section DownLockInv.
+  Context {oifc: OStateIfc}.
+  Variables (dtr: DTree)
+            (sys: System oifc).
+
+  Hypotheses (Hrr: GoodRqRsSys dtr sys)
+             (Hsd: RqRsDTree dtr sys).
+
+  Section OnMState.
+    Variables (orqs: ORqs Msg)
+              (msgs: MessagePool Msg).
+
+    Definition ODownLockedTo (oidx: IdxT) (rsbTo: IdxT) :=
+      orqs@[oidx] >>=[False]
+          (fun orq =>
+             exists rqi,
+               orq@[downRq] = Some rqi /\
+               rqi.(rqi_midx_rsb) = rsbTo).
+    
+    Definition ODownLockFree (oidx: IdxT) :=
+      orqs@[oidx] >>=[True] (fun orq => DownLockFreeORq orq).
+
+    Definition ONoDownLockTo (oidx: IdxT) (rsbTo: IdxT) :=
+      orqs@[oidx] >>=[True]
+          (fun orq =>
+             match orq@[downRq] with
+             | Some rqi => rqi.(rqi_midx_rsb) <> rsbTo
+             | None => True
+             end).
+    
+    Definition DownLockFreeInv (oidx: IdxT) :=
+      forall cidx,
+        parentIdxOf dtr cidx = Some oidx ->
+        exists down rsUp,
+          edgeDownTo dtr cidx = Some down /\ 
+          rsEdgeUpFrom dtr cidx = Some rsUp /\
+          rqsQ msgs down = nil /\
+          findQ rsUp msgs = nil /\
+          ONoDownLockTo cidx rsUp.
+
+    Definition DownLockedInv (oidx: IdxT) (rqi: RqInfo Msg) :=
+      Forall (fun rsUp =>
+                exists down cidx,
+                  edgeDownTo dtr cidx = Some down /\
+                  rsEdgeUpFrom dtr cidx = Some rsUp /\
+                  parentIdxOf dtr cidx = Some oidx /\
+                  length (rqsQ msgs down) <= 1 /\
+                  length (findQ rsUp msgs) <= 1 /\
+                  xor3 (length (rqsQ msgs down) = 1)
+                       (length (findQ rsUp msgs) = 1)
+                       (ODownLockedTo cidx rsUp))
+             rqi.(rqi_minds_rss).
+
+    Definition DownLockInvORq (oidx: IdxT) (orq: ORq Msg) :=
+      match orq@[downRq] with
+      | Some downRqi => DownLockedInv oidx downRqi
+      | None => DownLockFreeInv oidx
+      end.
+
+    Definition DownLockInvMO :=
+      forall oidx,
+        In oidx (map (@obj_idx _) sys.(sys_objs)) ->
+        let orq := orqs@[oidx] >>=[[]] (fun orq => orq) in
+        DownLockInvORq oidx orq.
+
+  End OnMState.
+  
+  Definition DownLockInv (st: MState oifc) :=
+    DownLockInvMO st.(bst_orqs) st.(bst_msgs).
+
+  Lemma downLockInv_init:
+    InvInit sys DownLockInv.
+  Proof.
+    intros; do 3 red; cbn.
+    intros; cbn.
+    red; intros.
+    eapply parentIdxOf_Some in H0; [|eassumption].
+    destruct H0 as [rqUp [rsUp [down ?]]]; dest.
+    exists down, rsUp; repeat split; assumption.
+  Qed.
+
+  Lemma downLockedInv_msgs_preserved:
+    forall orqs msgs1 msgs2 oidx rqi,
+      DownLockedInv orqs msgs1 oidx rqi ->
+      (forall rsUp down cidx,
+          In rsUp (rqi_minds_rss rqi) ->
+          edgeDownTo dtr cidx = Some down ->
+          rsEdgeUpFrom dtr cidx = Some rsUp ->
+          parentIdxOf dtr cidx = Some oidx ->
+          rqsQ msgs1 down = rqsQ msgs2 down /\
+          findQ rsUp msgs1 = findQ rsUp msgs2) ->
+      DownLockedInv orqs msgs2 oidx rqi.
+  Proof.
+    unfold DownLockedInv; simpl; intros.
+    rewrite Forall_forall in H.
+    apply Forall_forall; intros rsUp ?.
+    specialize (H _ H1).
+    destruct H as [down [cidx ?]]; dest.
+    specialize (H0 _ _ _ H1 H H2 H3); dest.
+    exists down, cidx.
+    rewrite <-H0, <-H7.
+    repeat split; try assumption.
+  Qed.
+  
+  Corollary downLockedInv_disj_enqMsgs_preserved:
+    forall orqs msgs emsgs oidx rqi,
+      DownLockedInv orqs msgs oidx rqi ->
+      DisjList (idsOf emsgs) (sys_minds sys) ->
+      DownLockedInv orqs (enqMsgs emsgs msgs) oidx rqi.
+  Proof.
+    intros.
+    eapply downLockedInv_msgs_preserved; eauto.
+    intros; split.
+    - unfold rqsQ.
+      rewrite findQ_not_In_enqMsgs; [reflexivity|].
+      eapply DisjList_In_1; [eassumption|].
+      eapply rqrsDTree_edgeDownTo_sys_minds; eauto.
+    - rewrite findQ_not_In_enqMsgs; [reflexivity|].
+      eapply DisjList_In_1; [eassumption|].
+      eapply rqrsDTree_rsEdgeUpFrom_sys_minds; eauto.
+  Qed.
+
+  Corollary downLockedInv_disj_deqMsgs_preserved:
+    forall orqs msgs eminds oidx rqi,
+      DownLockedInv orqs msgs oidx rqi ->
+      DisjList eminds (sys_minds sys) ->
+      DownLockedInv orqs (deqMsgs eminds msgs) oidx rqi.
+  Proof.
+    intros.
+    eapply downLockedInv_msgs_preserved; eauto.
+    intros; split.
+    - unfold rqsQ.
+      rewrite findQ_not_In_deqMsgs; [reflexivity|].
+      eapply DisjList_In_1; [eassumption|].
+      eapply rqrsDTree_edgeDownTo_sys_minds; eauto.
+    - rewrite findQ_not_In_deqMsgs; [reflexivity|].
+      eapply DisjList_In_1; [eassumption|].
+      eapply rqrsDTree_rsEdgeUpFrom_sys_minds; eauto.
+  Qed.
+
+  Lemma downLockFreeInv_msgs_preserved:
+    forall orqs msgs1 msgs2 oidx,
+      DownLockFreeInv orqs msgs1 oidx ->
+      (forall cidx,
+          parentIdxOf dtr cidx = Some oidx ->
+          (forall down,
+              edgeDownTo dtr cidx = Some down ->
+              rqsQ msgs1 down = rqsQ msgs2 down) /\
+          (forall rsUp,
+              rsEdgeUpFrom dtr cidx = Some rsUp ->
+              findQ rsUp msgs1 = findQ rsUp msgs2)) ->
+      DownLockFreeInv orqs msgs2 oidx.
+  Proof.
+    unfold DownLockFreeInv; simpl; intros.
+    specialize (H _ H1).
+    destruct H as [down [rsUp ?]]; dest.
+    specialize (H0 _ H1); destruct H0.
+    exists down, rsUp.
+    repeat split; auto.
+    - rewrite <-H0; auto.
+    - rewrite <-H6; auto.
+  Qed.
+  
+  Corollary downLockFreeInv_disj_enqMsgs_preserved:
+    forall orqs msgs emsgs oidx,
+      DownLockFreeInv orqs msgs oidx ->
+      DisjList (idsOf emsgs) (sys_minds sys) ->
+      DownLockFreeInv orqs (enqMsgs emsgs msgs) oidx.
+  Proof.
+    intros.
+    eapply downLockFreeInv_msgs_preserved; eauto.
+    intros; split; intros.
+    - unfold rqsQ.
+      rewrite findQ_not_In_enqMsgs; [reflexivity|].
+      eapply DisjList_In_1; [eassumption|].
+      eapply rqrsDTree_edgeDownTo_sys_minds; eauto.
+    - rewrite findQ_not_In_enqMsgs; [reflexivity|].
+      eapply DisjList_In_1; [eassumption|].
+      eapply rqrsDTree_rsEdgeUpFrom_sys_minds; eauto.
+  Qed.
+
+  Lemma downLockFreeInv_disj_deqMsgs_preserved:
+    forall orqs msgs eminds oidx,
+      DownLockFreeInv orqs msgs oidx ->
+      DisjList eminds (sys_minds sys) ->
+      DownLockFreeInv orqs (deqMsgs eminds msgs) oidx.
+  Proof.
+    intros.
+    eapply downLockFreeInv_msgs_preserved; eauto.
+    intros; split; intros.
+    - unfold rqsQ.
+      rewrite findQ_not_In_deqMsgs; [reflexivity|].
+      eapply DisjList_In_1; [eassumption|].
+      eapply rqrsDTree_edgeDownTo_sys_minds; eauto.
+    - rewrite findQ_not_In_deqMsgs; [reflexivity|].
+      eapply DisjList_In_1; [eassumption|].
+      eapply rqrsDTree_rsEdgeUpFrom_sys_minds; eauto.
+  Qed.
+
+  Corollary downLockedInv_orqs_preserved_self_update:
+    forall orqs msgs oidx orq rqid,
+      DownLockedInv orqs msgs oidx rqid ->
+      DownLockedInv (orqs+[oidx <- orq]) msgs oidx rqid.
+  Proof.
+    intros.
+    destruct Hsd.
+    red in H; red.
+    eapply Forall_impl; [|eassumption].
+    clear H; simpl; intro midx; intros.
+    destruct H as [down [cidx ?]]; dest.
+    exists down, cidx.
+    repeat split; try assumption.
+    unfold ODownLockedTo in *.
+    apply parentIdxOf_not_eq in H3; [|assumption].
+    mred.
+  Qed.
+
+  Lemma downLockFreeInv_orqs_preserved_self_update:
+    forall orqs msgs oidx orq,
+      DownLockFreeInv orqs msgs oidx ->
+      DownLockFreeInv (orqs+[oidx <- orq]) msgs oidx.
+  Proof.
+    unfold DownLockFreeInv; intros; dest.
+    specialize (H _ H0).
+    destruct H as [down [rsUp ?]]; dest.
+    exists down, rsUp.
+    repeat split; try assumption.
+    red in H4; red.
+    apply parentIdxOf_not_eq in H0; [|destruct Hsd; assumption].
+    mred.
+  Qed.
+
+  Lemma downLockInv_step_ext_in:
+    forall oss orqs msgs eins,
+      DownLockInv {| bst_oss := oss; bst_orqs := orqs; bst_msgs := msgs |} ->
+      eins <> nil ->
+      ValidMsgsExtIn sys eins ->
+      DownLockInv {| bst_oss := oss;
+                     bst_orqs := orqs;
+                     bst_msgs := enqMsgs eins msgs |}.
+  Proof.
+    unfold DownLockInv; simpl; intros.
+    red; intros.
+    specialize (H oidx H2).
+    destruct H1.
+    assert (DisjList (idsOf eins) (sys_minds sys)).
+    { eapply DisjList_SubList; eauto.
+      apply DisjList_comm.
+      apply sys_minds_sys_merqs_DisjList.
+    }
+    destruct (orqs@[oidx]) as [orq|]; simpl in *; dest.
+    - red in H; red.
+      remember (orq@[downRq]) as orqi.
+      destruct orqi as [rqi|].
+      + apply downLockedInv_disj_enqMsgs_preserved; assumption.
+      + apply downLockFreeInv_disj_enqMsgs_preserved; assumption.
+    - red in H; simpl in H.
+      red in H3; simpl in H3.
+      red; simpl.
+      apply downLockFreeInv_disj_enqMsgs_preserved; assumption.
+  Qed.
+
+  Lemma downLockInv_step_ext_out:
+    forall oss orqs msgs eouts,
+      DownLockInv {| bst_oss := oss; bst_orqs := orqs; bst_msgs := msgs |} ->
+      eouts <> nil ->
+      Forall (FirstMPI msgs) eouts ->
+      ValidMsgsExtOut sys eouts ->
+      DownLockInv {| bst_oss := oss;
+                     bst_orqs := orqs;
+                     bst_msgs := deqMsgs (idsOf eouts) msgs |}.
+  Proof.
+    unfold DownLockInv; simpl; intros.
+    red; intros.
+    specialize (H oidx H3).
+    destruct H2.
+    assert (DisjList (idsOf eouts) (sys_minds sys)).
+    { eapply DisjList_SubList; eauto.
+      apply DisjList_comm.
+      apply sys_minds_sys_merss_DisjList.
+    }
+    destruct (orqs@[oidx]) as [orq|]; simpl in *; dest.
+    - red in H; red.
+      remember (orq@[downRq]) as orqi.
+      destruct orqi as [rqi|].
+      + apply downLockedInv_disj_deqMsgs_preserved; assumption.
+      + apply downLockFreeInv_disj_deqMsgs_preserved; assumption.
+    - red in H; simpl in H.
+      red in H4; simpl in H4.
+      red; simpl.
+      apply downLockFreeInv_disj_deqMsgs_preserved; assumption.
+  Qed.
+
+  Section InternalStep.
+    Variables (oss: OStates oifc) (orqs: ORqs Msg) (msgs: MessagePool Msg)
+              (obj: Object oifc) (rule: Rule oifc)
+              (post: OState oifc) (porq: ORq Msg) (mins: list (Id Msg))
+              (nost: OState oifc) (norq: ORq Msg) (mouts: list (Id Msg)).
+
+    Hypotheses
+      (Hfpok: FootprintsOk
+                dtr sys {| bst_oss := oss; bst_orqs := orqs; bst_msgs := msgs |})
+      (HobjIn: In obj (sys_objs sys))
+      (HruleIn: In rule (obj_rules obj))
+      (Hporq: orqs@[obj_idx obj] = Some porq)
+      (Hpost: oss@[obj_idx obj] = Some post)
+      (HminsF: Forall (FirstMPI msgs) mins)
+      (HminsV: ValidMsgsIn sys mins)
+      (Hprec: rule_precond rule post porq mins)
+      (Htrs: rule_trs rule post porq mins = (nost, norq, mouts))
+      (HmoutsV: ValidMsgsOut sys mouts)
+      (Hmdisj: DisjList (idsOf mins) (idsOf mouts)).
+
+    Ltac disc_rule_custom ::=
+      match goal with
+      | [H: FootprintUpOkEx _ _ _ /\ _ |- _] => destruct H
+      | [H: _ /\ FootprintDownOkEx _ _ _ _ |- _] => destruct H
+      | [H: FootprintUpOkEx _ _ _ |- _] =>
+        let rqFrom := fresh "rqFrom" in
+        let rqTo := fresh "rqTo" in
+        let rsFrom := fresh "rsFrom" in
+        let rsbTo := fresh "rsbTo" in
+        destruct H as [rqFrom [rqTo [rsFrom [rsbTo ?]]]]; dest
+      | [H: FootprintUpOk _ _ _ _ _ _ |- _] =>
+        let cidx := fresh "cidx" in
+        destruct H as [cidx ?]; dest
+
+      | [H: FootprintDownOkEx _ _ _ _ |- _] =>
+        let rqFrom := fresh "rqFrom" in
+        let rqTos := fresh "rqTos" in
+        let rssFrom := fresh "rssFrom" in
+        let rsbTo := fresh "rsbTo" in
+        destruct H as [rqFrom [rqTos [rssFrom [rsbTo ?]]]]; dest
+      | [H: FootprintUpDownOk _ _ _ _ _ _ _ \/
+            FootprintDownDownOk _ _ _ _ _ _ |- _] => destruct H
+      | [H: exists _, FootprintUpDownOk _ _ _ _ _ _ _ |- _] =>
+        let rqFrom := fresh "rqFrom" in
+        destruct H as [rqFrom ?]
+      | [H: FootprintUpDownOk _ _ _ _ _ _ _ |- _] =>
+        let upCIdx := fresh "upCIdx" in
+        let upCObj := fresh "upCObj" in
+        destruct H as [upCIdx [upCObj ?]]; dest
+      | [H: FootprintDownDownOk _ _ _ _ _ _ |- _] => red in H; dest
+      end.
+
+    Lemma downLockInvORq_step_int_me:
+      DownLockInvORq orqs msgs (obj_idx obj) porq ->
+      In (obj_idx obj) (map (@obj_idx _) (sys_objs sys)) ->
+      GoodRqRsRule dtr sys (obj_idx obj) rule ->
+      DownLockInvORq (orqs+[obj_idx obj <- norq])
+                     (enqMsgs mouts (deqMsgs (idsOf mins) msgs))
+                     (obj_idx obj) norq.
+    Proof.
+      intros.
+      destruct Hsd.
+      red in H; red.
+      good_rqrs_rule_cases rule.
+
+      - (** case [ImmDownRule] *)
+        disc_rule_conds.
+        apply downLockFreeInv_orqs_preserved_self_update.
+        eapply downLockFreeInv_msgs_preserved; eauto.
+        intros; split; intros.
+        + rewrite rqsQ_enqMP_rs by assumption.
+          solve_q.
+        + solve_q.
+
+      - (** case [ImmUpRule] *)
+        disc_rule_conds.
+        apply downLockFreeInv_orqs_preserved_self_update.
+        eapply downLockFreeInv_msgs_preserved; eauto.
+        intros; split; intros; solve_q.
+
+      - (** case [RqFwdRule] *)
+        disc_rule_conds.
+        + (** case [RqUpUp] *)
+          destruct (porq@[downRq]) as [rqid|].
+          * apply downLockedInv_orqs_preserved_self_update.
+            eapply downLockedInv_msgs_preserved; eauto.
+            intros; split; intros; solve_q.
+          * apply downLockFreeInv_orqs_preserved_self_update.
+            eapply downLockFreeInv_msgs_preserved; eauto.
+            intros; split; intros; solve_q.
+        + (** case [RqUpDown] *)
+          apply downLockedInv_orqs_preserved_self_update.
+          admit.
+        + (** case [RqDownDown] *)
+          apply downLockedInv_orqs_preserved_self_update.
+          admit.
+
+      - (** case [RsBackRule] *)
+        good_footprint_get (obj_idx obj).
+        disc_rule_conds.
+        + (** case [RsDownDown] *)
+          apply downLockFreeInv_orqs_preserved_self_update.
+          eapply downLockFreeInv_msgs_preserved; eauto.
+          intros; split; intros.
+          * rewrite rqsQ_enqMP_rs by assumption.
+            solve_q.
+          * solve_q.
+        + (** case [RsUp(Down)] *)
+          apply downLockFreeInv_orqs_preserved_self_update.
+          admit.
+        + (** case [RsUp(Up)] *)
+          apply downLockFreeInv_orqs_preserved_self_update.
+          admit.
+
+      - (** case [RsDownRqDownRule] *)
+        disc_rule_conds.
+        apply downLockedInv_orqs_preserved_self_update.
+        admit.
+      
+    Admitted.
+
+    Lemma downLockInvORq_step_int_other:
+      forall oidx,
+        DownLockInvORq orqs msgs oidx ((orqs@[oidx]) >>=[[]] (fun orq => orq)) ->
+        In oidx (map (@obj_idx _) (sys_objs sys)) ->
+        GoodRqRsRule dtr sys (obj_idx obj) rule ->
+        obj_idx obj <> oidx ->
+        DownLockInvORq (orqs+[obj_idx obj <- norq])
+                     (enqMsgs mouts (deqMsgs (idsOf mins) msgs)) oidx
+                     ((orqs@[ oidx]) >>=[[]] (fun orq => orq)).
+    Proof.
+    Admitted.
+
+    Lemma downLockInv_step_int:
+      DownLockInv {| bst_oss := oss; bst_orqs := orqs; bst_msgs := msgs |} ->
+      DownLockInv {| bst_oss := (oss) +[ obj_idx obj <- nost];
+                     bst_orqs := (orqs) +[ obj_idx obj <- norq];
+                     bst_msgs := enqMsgs mouts (deqMsgs (idsOf mins) msgs) |}.
+    Proof.
+      intros.
+      do 2 red; simpl; intros.
+      good_rqrs_rule_get rule.
+      specialize (H _ H0); simpl in H; dest.
+
+      M.cmp (obj_idx obj) oidx; mred; simpl in *.
+      - (** case [oidx = obj_idx obj] *)
+        apply downLockInvORq_step_int_me; assumption.
+      - (** case [oidx <> obj_idx obj] *)
+        apply downLockInvORq_step_int_other; assumption.
+    Qed.
+
+  End InternalStep.
+
+  Lemma downLockInv_step:
+    InvStep sys step_m DownLockInv.
+  Proof.
+    red; intros.
+    inv H1.
+    - auto.
+    - apply downLockInv_step_ext_in; auto.
+    - apply downLockInv_step_ext_out; auto.
+    - eapply downLockInv_step_int; eauto.
+      eapply footprints_ok; eassumption.
+  Qed.
+
+  Lemma downLockInv_ok:
+    InvReachable sys step_m DownLockInv.
+  Proof.
+    apply inv_reachable.
+    - apply downLockInv_init.
+    - apply downLockInv_step.
+  Qed.
+  
+End DownLockInv.
+
+Close Scope list.
+Close Scope fmap.
+
