src/RqRsInvUpLock.v
@@ -1,0 +1,2330 @@
+Require Import Peano_dec Omega List ListSupport.
+Require Import Common FMap.
+Require Import Syntax Semantics SemFacts StepM Invariant Serial.
+Require Import Reduction Commutativity QuasiSeq Topology.
+Require Import RqRsTopo RqRsFacts RqRsInvMsg.
+
+Set Implicit Arguments.
+
+Open Scope list.
+Open Scope fmap.
+
+Section UpLockInv.
+  Context {oifc: OStateIfc}.
+  Variables (dtr: DTree)
+            (sys: System oifc).
+
+  Hypotheses (Hrr: GoodRqRsSys dtr sys)
+             (Hsd: RqRsDTree dtr sys).
+
+  Section OnMState.
+    Variables (orqs: ORqs Msg)
+              (msgs: MessagePool Msg).
+
+    Definition OLockedTo (oidx: IdxT) (rsbTo: IdxT) :=
+      orqs@[oidx] >>=[False]
+          (fun orq =>
+             exists rqi,
+               (orq@[upRq] = Some rqi \/ orq@[downRq] = Some rqi) /\
+               rqi.(rqi_midx_rsb) = rsbTo).
+
+    Definition ONoSameLockTo (oidx: IdxT) (rsbTo: IdxT) :=
+      orqs@[oidx] >>=[True]
+          (fun orq =>
+             match orq@[upRq], orq@[downRq] with
+             | Some rqiu, Some rqid =>
+               rqiu.(rqi_midx_rsb) <> rsbTo \/ rqid.(rqi_midx_rsb) <> rsbTo
+             | _, _ => True
+             end).
+
+    Definition OUpLockFree (oidx: IdxT) :=
+      orqs@[oidx] >>=[True] (fun orq => UpLockFreeORq orq).
+
+    Definition ONoLockTo (oidx: IdxT) (rsbTo: IdxT) :=
+      orqs@[oidx] >>=[True]
+          (fun orq =>
+             match orq@[upRq] with
+             | Some rqi => rqi.(rqi_midx_rsb) <> rsbTo
+             | None => True
+             end /\
+             match orq@[downRq] with
+             | Some rqi => rqi.(rqi_midx_rsb) <> rsbTo
+             | None => True
+             end).
+
+    Definition UpLockFreeInv (oidx: IdxT) :=
+      parentIdxOf dtr oidx = None \/
+      exists rqUp down pidx,
+        rqEdgeUpFrom dtr oidx = Some rqUp /\
+        edgeDownTo dtr oidx = Some down /\
+        parentIdxOf dtr oidx = Some pidx /\
+        findQ rqUp msgs = nil /\
+        rssQ msgs down = nil /\
+        ONoLockTo pidx down.
+    
+    Definition UpLockedInv (oidx: IdxT) :=
+      exists rqUp down pidx,
+        rqEdgeUpFrom dtr oidx = Some rqUp /\
+        edgeDownTo dtr oidx = Some down /\
+        parentIdxOf dtr oidx = Some pidx /\
+        length (findQ rqUp msgs) <= 1 /\
+        length (rssQ msgs down) <= 1 /\
+        ONoSameLockTo pidx down /\
+        xor3 (length (findQ rqUp msgs) = 1)
+             (length (rssQ msgs down) = 1)
+             (OLockedTo pidx down).
+
+    Definition UpLockInvORq (oidx: IdxT) (orq: ORq Msg) :=
+      match orq@[upRq] with
+      | Some _ => UpLockedInv oidx
+      | None => UpLockFreeInv oidx
+      end.
+
+    Definition UpLockInvMO :=
+      forall oidx,
+        In oidx (map (@obj_idx _) sys.(sys_objs)) ->
+        let orq := orqs@[oidx] >>=[[]] (fun orq => orq) in
+        UpLockInvORq oidx orq.
+
+  End OnMState.
+  
+  Definition UpLockInv (st: MState oifc) :=
+    UpLockInvMO st.(bst_orqs) st.(bst_msgs).
+
+  Lemma upLockInv_init:
+    InvInit sys UpLockInv.
+  Proof.
+    intros; do 3 red; cbn.
+    intros; cbn.
+    red.
+    remember (parentIdxOf dtr oidx) as opidx.
+    destruct opidx as [pidx|]; [right|left; reflexivity].
+    pose proof (eq_sym Heqopidx).
+    eapply parentIdxOf_Some in H0; [|eassumption].
+    destruct H0 as [rqUp [rsUp [down ?]]]; dest.
+    do 3 eexists; repeat split; try eassumption.
+  Qed.
+
+  Lemma ONoLockTo_not_OLockedTo:
+    forall orqs oidx rsbTo,
+      ONoLockTo orqs oidx rsbTo -> ~ OLockedTo orqs oidx rsbTo.
+  Proof.
+    unfold ONoLockTo, OLockedTo; intros.
+    intro Hx.
+    destruct (orqs@[oidx]); simpl in *; auto; dest.
+    destruct H1.
+    - rewrite H1 in H; auto.
+    - rewrite H1 in H0; auto.
+  Qed.
+
+  Lemma not_ONoLockTo_OLockedTo:
+    forall orqs oidx rsbTo,
+      ~ OLockedTo orqs oidx rsbTo -> ONoLockTo orqs oidx rsbTo.
+  Proof.
+    unfold ONoLockTo, OLockedTo; intros.
+    destruct (orqs@[oidx]); simpl in *; auto.
+    split.
+    - destruct (o@[upRq]); auto.
+      intro Hx; elim H.
+      eexists; split; eauto.
+    - destruct (o@[downRq]); auto.
+      intro Hx; elim H.
+      eexists; split; eauto.
+  Qed.
+
+  Lemma ONoLockTo_ONoSameLockTo:
+    forall orqs oidx rsbTo,
+      ONoLockTo orqs oidx rsbTo -> ONoSameLockTo orqs oidx rsbTo.
+  Proof.
+    unfold ONoLockTo, ONoSameLockTo; intros.
+    destruct (orqs@[oidx]) as [orq|]; simpl in *; auto.
+    destruct (orq@[upRq]) as [rqiu|]; simpl in *; auto.
+    dest.
+    destruct (orq@[downRq]) as [rqid|]; simpl in *; auto.
+  Qed.
+
+  Lemma OLockedTo_orqs_preserved:
+    forall orqs1 orqs2 oidx rsbTo,
+      OLockedTo orqs1 oidx rsbTo ->
+      orqs1@[oidx] = orqs2@[oidx] ->
+      OLockedTo orqs2 oidx rsbTo.
+  Proof.
+    unfold OLockedTo; intros.
+    rewrite <-H0; assumption.
+  Qed.
+
+  Lemma upLockedInv_msgs_preserved:
+    forall orqs msgs1 msgs2 oidx,
+      UpLockedInv orqs msgs1 oidx ->
+      (match rqEdgeUpFrom dtr oidx with
+       | Some rqUp => findQ rqUp msgs1 = findQ rqUp msgs2
+       | None => False
+       end) ->
+      (match edgeDownTo dtr oidx with
+       | Some down => rssQ msgs1 down = rssQ msgs2 down
+       | None => False
+       end) ->
+      UpLockedInv orqs msgs2 oidx.
+  Proof.
+    unfold UpLockedInv; simpl; intros.
+    destruct H as [rqUp [down [pidx ?]]]; dest.
+    rewrite H in H0.
+    rewrite H2 in H1.
+    exists rqUp, down, pidx.
+    rewrite <-H0, <-H1.
+    repeat split; try assumption.
+  Qed.
+
+  Corollary upLockedInv_disj_enqMsgs_preserved:
+    forall orqs msgs emsgs oidx,
+      UpLockedInv orqs msgs oidx ->
+      DisjList (idsOf emsgs) (sys_minds sys) ->
+      UpLockedInv orqs (enqMsgs emsgs msgs) oidx.
+  Proof.
+    intros.
+    eapply upLockedInv_msgs_preserved; eauto.
+    - destruct H as [rqUp [down [pidx ?]]]; dest.
+      rewrite H.
+      rewrite findQ_not_In_enqMsgs.
+      + reflexivity.
+      + eapply DisjList_In_1; [eassumption|].
+        eapply rqrsDTree_rqEdgeUpFrom_sys_minds; eauto.
+    - destruct H as [rqUp [down [pidx ?]]]; dest.
+      rewrite H1.
+      unfold rssQ.
+      rewrite findQ_not_In_enqMsgs.
+      + reflexivity.
+      + eapply DisjList_In_1; [eassumption|].
+        eapply rqrsDTree_edgeDownTo_sys_minds; eauto.
+  Qed.
+
+  Corollary upLockedInv_disj_deqMsgs_preserved:
+    forall orqs msgs eminds oidx,
+      UpLockedInv orqs msgs oidx ->
+      DisjList eminds (sys_minds sys) ->
+      UpLockedInv orqs (deqMsgs eminds msgs) oidx.
+  Proof.
+    intros.
+    eapply upLockedInv_msgs_preserved; eauto.
+    - destruct H as [rqUp [down [pidx ?]]]; dest.
+      rewrite H.
+      rewrite findQ_not_In_deqMsgs.
+      + reflexivity.
+      + eapply DisjList_In_1; [eassumption|].
+        eapply rqrsDTree_rqEdgeUpFrom_sys_minds; eauto.
+    - destruct H as [rqUp [down [pidx ?]]]; dest.
+      rewrite H1.
+      unfold rssQ.
+      rewrite findQ_not_In_deqMsgs.
+      + reflexivity.
+      + eapply DisjList_In_1; [eassumption|].
+        eapply rqrsDTree_edgeDownTo_sys_minds; eauto.
+  Qed.
+
+  Lemma upLockFreeInv_msgs_preserved:
+    forall orqs msgs1 msgs2 oidx,
+      UpLockFreeInv orqs msgs1 oidx ->
+      (match rqEdgeUpFrom dtr oidx with
+       | Some rqUp => findQ rqUp msgs1 = findQ rqUp msgs2
+       | None => True
+       end) ->
+      (match edgeDownTo dtr oidx with
+       | Some down => rssQ msgs1 down = rssQ msgs2 down
+       | None => True
+       end) ->
+      UpLockFreeInv orqs msgs2 oidx.
+  Proof.
+    unfold UpLockFreeInv; simpl; intros.
+    destruct H; [left; assumption|right].
+    destruct H as [rqUp [down [pidx ?]]]; dest.
+    rewrite H in H0.
+    rewrite H2 in H1.
+    exists rqUp, down, pidx; repeat split;
+      try assumption; try congruence.
+  Qed.
+
+  Corollary upLockFreeInv_disj_enqMsgs_preserved:
+    forall orqs msgs emsgs oidx,
+      UpLockFreeInv orqs msgs oidx ->
+      DisjList (idsOf emsgs) (sys_minds sys) ->
+      UpLockFreeInv orqs (enqMsgs emsgs msgs) oidx.
+  Proof.
+    intros.
+    eapply upLockFreeInv_msgs_preserved; eauto.
+    - red in H; dest.
+      remember (rqEdgeUpFrom dtr oidx) as rqUp.
+      destruct rqUp as [rqUp|]; simpl in *; dest; auto.
+      rewrite findQ_not_In_enqMsgs.
+      + reflexivity.
+      + eapply DisjList_In_1; [eassumption|].
+        eapply rqrsDTree_rqEdgeUpFrom_sys_minds; eauto.
+    - red in H; dest.
+      remember (edgeDownTo dtr oidx) as down.
+      destruct down as [down|]; simpl in *; dest; auto.
+      unfold rssQ.
+      rewrite findQ_not_In_enqMsgs.
+      + reflexivity.
+      + eapply DisjList_In_1; [eassumption|].
+        eapply rqrsDTree_edgeDownTo_sys_minds; eauto.
+  Qed.
+
+  Corollary upLockFreeInv_disj_deqMsgs_preserved:
+    forall orqs msgs eminds oidx,
+      UpLockFreeInv orqs msgs oidx ->
+      DisjList eminds (sys_minds sys) ->
+      UpLockFreeInv orqs (deqMsgs eminds msgs) oidx.
+  Proof.
+    intros.
+    eapply upLockFreeInv_msgs_preserved; eauto.
+    - red in H; dest.
+      remember (rqEdgeUpFrom dtr oidx) as rqUp.
+      destruct rqUp as [rqUp|]; simpl in *; dest; auto.
+      rewrite findQ_not_In_deqMsgs.
+      + reflexivity.
+      + eapply DisjList_In_1; [eassumption|].
+        eapply rqrsDTree_rqEdgeUpFrom_sys_minds; eauto.
+    - red in H; dest.
+      remember (edgeDownTo dtr oidx) as down.
+      destruct down as [down|]; simpl in *; dest; auto.
+      unfold rssQ.
+      rewrite findQ_not_In_deqMsgs.
+      + reflexivity.
+      + eapply DisjList_In_1; [eassumption|].
+        eapply rqrsDTree_edgeDownTo_sys_minds; eauto.
+  Qed.
+
+  Lemma upLockedInv_orqs_preserved_parent_eq:
+    forall (orqs1 orqs2: ORqs Msg) msgs oidx pidx,
+      UpLockedInv orqs1 msgs oidx ->
+      parentIdxOf dtr oidx = Some pidx ->
+      orqs1@[pidx] = orqs2@[pidx] ->
+      UpLockedInv orqs2 msgs oidx.
+  Proof.
+    unfold UpLockedInv; intros.
+    destruct H as [rqUp [down [pidx' ?]]]; dest.
+    rewrite H3 in H0; inv H0.
+    exists rqUp, down, pidx; repeat split; try assumption.
+    - red in H6; red; rewrite <-H1; assumption.
+    - unfold OLockedTo in *; rewrite <-H1; assumption.
+  Qed.
+
+  Corollary upLockedInv_orqs_preserved_self_update:
+    forall orqs msgs oidx orq,
+      UpLockedInv orqs msgs oidx ->
+      UpLockedInv (orqs+[oidx <- orq]) msgs oidx.
+  Proof.
+    intros.
+    destruct Hsd.
+    pose proof H.
+    destruct H2 as [rqUp [down [pidx ?]]]; dest.
+    eapply upLockedInv_orqs_preserved_parent_eq; eauto.
+    apply parentIdxOf_not_eq in H4; [|assumption].
+    mred.
+  Qed.
+
+  Lemma upLockedInv_orqs_preserved_parent_some_up:
+    forall (orqs1 orqs2: ORqs Msg) msgs oidx pidx rqiu,
+      UpLockedInv orqs1 msgs oidx ->
+      parentIdxOf dtr oidx = Some pidx ->
+      orqs1@[pidx] >>= (fun orq1 => orq1@[upRq]) = None ->
+      orqs2@[pidx] >>= (fun orq2 => orq2@[upRq]) = Some rqiu ->
+      edgeDownTo dtr oidx <> Some (rqiu.(rqi_midx_rsb)) ->
+      orqs1@[pidx] >>= (fun orq1 => orq1@[downRq]) =
+      orqs2@[pidx] >>= (fun orq2 => orq2@[downRq]) ->
+      UpLockedInv orqs2 msgs oidx.
+  Proof.
+    unfold UpLockedInv; intros.
+    destruct H as [rqUp [down [pidx' ?]]]; dest.
+    rewrite H6 in H0; inv H0.
+    exists rqUp, down, pidx; repeat split; try assumption.
+
+    - red in H9; red.
+      destruct (orqs1@[pidx]) as [orq1|];
+        destruct (orqs2@[pidx]) as [orq2|]; simpl in *;
+          try (exfalso; auto; fail); try discriminate.
+      + rewrite H2.
+        destruct (orq2@[downRq]) as [rqid2|]; auto.
+        rewrite H5 in H3.
+        left; intro Hx; subst; auto.
+      + rewrite H2, <-H4; auto.
+    
+    - destruct H10.
+      + xfst; try assumption.
+        intro Hx; red in Hx.
+        destruct (orqs2@[pidx]) as [orq2|]; simpl in *; auto.
+        destruct Hx as [rqi ?]; dest.
+        destruct H12.
+        * rewrite H2 in H12; inv H12.
+          elim H3; assumption.
+        * elim H11; red.
+          destruct (orqs1@[pidx]) as [orq1|]; simpl in *; auto.
+          { eexists; split.
+            { right; rewrite H4; eassumption. }
+            { assumption. }
+          }
+          { congruence. }
+      + xsnd; try assumption.
+        intro Hx; red in Hx.
+        destruct (orqs2@[pidx]) as [orq2|]; simpl in *; auto.
+        destruct Hx as [rqi ?]; dest.
+        destruct H12.
+        * rewrite H2 in H12; inv H12.
+          elim H3; assumption.
+        * elim H11; red.
+          destruct (orqs1@[pidx]) as [orq1|]; simpl in *; auto.
+          { eexists; split.
+            { right; rewrite H4; eassumption. }
+            { assumption. }
+          }
+          { congruence. }
+      + xthd; try assumption.
+        red; red in H11.
+        destruct (orqs2@[pidx]) as [orq2|]; simpl in *.
+        * destruct (orqs1@[pidx]) as [orq1|]; simpl in *.
+          { destruct H11 as [rqi ?]; dest.
+            destruct H11.
+            { congruence. }
+            { eexists; split.
+              { right; rewrite <-H4; eassumption. }
+              { assumption. }
+            }
+          }
+          { elim H11. }
+        * discriminate.
+  Qed.
+
+  Lemma upLockedInv_orqs_preserved_parent_some_down:
+    forall (orqs1 orqs2: ORqs Msg) msgs oidx pidx rqiu,
+      UpLockedInv orqs1 msgs oidx ->
+      parentIdxOf dtr oidx = Some pidx ->
+      orqs1@[pidx] >>= (fun orq1 => orq1@[downRq]) = None ->
+      orqs2@[pidx] >>= (fun orq2 => orq2@[downRq]) = Some rqiu ->
+      edgeDownTo dtr oidx <> Some (rqiu.(rqi_midx_rsb)) ->
+      orqs1@[pidx] >>= (fun orq1 => orq1@[upRq]) =
+      orqs2@[pidx] >>= (fun orq2 => orq2@[upRq]) ->
+      UpLockedInv orqs2 msgs oidx.
+  Proof.
+    unfold UpLockedInv; intros.
+    destruct H as [rqUp [down [pidx' ?]]]; dest.
+    rewrite H6 in H0; inv H0.
+    exists rqUp, down, pidx; repeat split; try assumption.
+    - red in H9; red.
+      destruct (orqs1@[pidx]) as [orq1|];
+        destruct (orqs2@[pidx]) as [orq2|]; simpl in *;
+          try (exfalso; auto; fail); try discriminate.
+      + rewrite <-H4.
+        destruct (orq1@[upRq]) as [rqiu1|]; auto.
+        rewrite H2.
+        right; intro Hx; subst; auto.
+      + rewrite H2, <-H4; auto.
+
+    - destruct H10.
+      + xfst; try assumption.
+        intro Hx; red in Hx.
+        destruct (orqs2@[pidx]) as [orq2|]; simpl in *; auto.
+        destruct Hx as [rqi ?]; dest.
+        destruct H12.
+        * elim H11; red.
+          destruct (orqs1@[pidx]) as [orq1|]; simpl in *; auto.
+          { eexists; split.
+            { left; rewrite H4; eassumption. }
+            { assumption. }
+          }
+          { congruence. }
+        * rewrite H2 in H12; inv H12.
+          elim H3; assumption.
+      + xsnd; try assumption.
+        intro Hx; red in Hx.
+        destruct (orqs2@[pidx]) as [orq2|]; simpl in *; auto.
+        destruct Hx as [rqi ?]; dest.
+        destruct H12.
+        * elim H11; red.
+          destruct (orqs1@[pidx]) as [orq1|]; simpl in *; auto.
+          { eexists; split.
+            { left; rewrite H4; eassumption. }
+            { assumption. }
+          }
+          { congruence. }
+        * rewrite H2 in H12; inv H12.
+          elim H3; assumption.
+      + xthd; try assumption.
+        red; red in H11.
+        destruct (orqs2@[pidx]) as [orq2|]; simpl in *; auto.
+        * destruct (orqs1@[pidx]) as [orq1|]; simpl in *.
+          { destruct H11 as [rqi ?]; dest.
+            destruct H11.
+            { eexists; split.
+              { left; rewrite <-H4; eassumption. }
+              { assumption. }
+            }
+            { congruence. }
+          }
+          { elim H11. }
+        * discriminate.
+  Qed.
+
+  Lemma upLockedInv_orqs_preserved_parent_none_up:
+    forall (orqs1 orqs2: ORqs Msg) msgs oidx pidx rqiu,
+      UpLockedInv orqs1 msgs oidx ->
+      parentIdxOf dtr oidx = Some pidx ->
+      orqs1@[pidx] >>= (fun orq1 => orq1@[upRq]) = Some rqiu ->
+      orqs2@[pidx] >>= (fun orq2 => orq2@[upRq]) = None ->
+      edgeDownTo dtr oidx <> Some (rqiu.(rqi_midx_rsb)) ->
+      orqs1@[pidx] >>= (fun orq1 => orq1@[downRq]) =
+      orqs2@[pidx] >>= (fun orq2 => orq2@[downRq]) ->
+      UpLockedInv orqs2 msgs oidx.
+  Proof.
+    unfold UpLockedInv; intros.
+    destruct H as [rqUp [down [pidx' ?]]]; dest.
+    rewrite H6 in H0; inv H0.
+    exists rqUp, down, pidx; repeat split; try assumption.
+    - red in H9; red.
+      destruct (orqs1@[pidx]) as [orq1|];
+        destruct (orqs2@[pidx]) as [orq2|]; simpl in *;
+          auto; try discriminate.
+      rewrite H2; auto.
+    - destruct H10.
+      + xfst; try assumption.
+        intro Hx; elim H11; clear H11.
+        red in Hx; red.
+        destruct (orqs1@[pidx]) as [orq1|];
+          destruct (orqs2@[pidx]) as [orq2|]; simpl in *; auto;
+            try discriminate.
+        * destruct Hx as [rqi ?]; dest.
+          destruct H11; [congruence|].
+          exists rqi; split; auto.
+          right; congruence.
+        * exfalso; auto.
+      + xsnd; try assumption.
+        intro Hx; elim H11; clear H11.
+        red in Hx; red.
+        destruct (orqs1@[pidx]) as [orq1|];
+          destruct (orqs2@[pidx]) as [orq2|]; simpl in *; auto;
+            try discriminate.
+        * destruct Hx as [rqi ?]; dest.
+          destruct H11; [congruence|].
+          exists rqi; split; auto.
+          right; congruence.
+        * exfalso; auto.
+      + xthd; try assumption.
+        red; red in H11.
+        destruct (orqs1@[pidx]) as [orq1|];
+          destruct (orqs2@[pidx]) as [orq2|]; simpl in *; auto;
+            try discriminate.
+        * destruct H11 as [rqi ?]; dest.
+          destruct H11; [congruence|].
+          eexists; split.
+          { right; rewrite <-H4; eassumption. }
+          { assumption. }
+        * destruct H11 as [rqi ?]; dest.
+          destruct H11; [|congruence].
+          subst; rewrite H11 in H1; inv H1.
+          auto.
+  Qed.
+
+  Lemma upLockedInv_orqs_preserved_parent_none_down:
+    forall (orqs1 orqs2: ORqs Msg) msgs oidx pidx rqiu,
+      UpLockedInv orqs1 msgs oidx ->
+      parentIdxOf dtr oidx = Some pidx ->
+      orqs1@[pidx] >>= (fun orq1 => orq1@[downRq]) = Some rqiu ->
+      orqs2@[pidx] >>= (fun orq2 => orq2@[downRq]) = None ->
+      edgeDownTo dtr oidx <> Some (rqiu.(rqi_midx_rsb)) ->
+      orqs1@[pidx] >>= (fun orq1 => orq1@[upRq]) =
+      orqs2@[pidx] >>= (fun orq2 => orq2@[upRq]) ->
+      UpLockedInv orqs2 msgs oidx.
+  Proof.
+    unfold UpLockedInv; intros.
+    destruct H as [rqUp [down [pidx' ?]]]; dest.
+    rewrite H6 in H0; inv H0.
+    exists rqUp, down, pidx; repeat split; try assumption.
+    - red in H9; red.
+      destruct (orqs1@[pidx]) as [orq1|];
+        destruct (orqs2@[pidx]) as [orq2|]; simpl in *;
+          auto; try discriminate.
+      rewrite H2.
+      destruct (orq2@[upRq]); auto.
+    - destruct H10.
+      + xfst; try assumption.
+        intro Hx; elim H11; clear H11.
+        red in Hx; red.
+        destruct (orqs1@[pidx]) as [orq1|];
+          destruct (orqs2@[pidx]) as [orq2|]; simpl in *; auto;
+            try discriminate.
+        * destruct Hx as [rqi ?]; dest.
+          destruct H11; [|congruence].
+          exists rqi; split; auto.
+          left; congruence.
+        * exfalso; auto.
+      + xsnd; try assumption.
+        intro Hx; elim H11; clear H11.
+        red in Hx; red.
+        destruct (orqs1@[pidx]) as [orq1|];
+          destruct (orqs2@[pidx]) as [orq2|]; simpl in *; auto;
+            try discriminate.
+        * destruct Hx as [rqi ?]; dest.
+          destruct H11; [|congruence].
+          exists rqi; split; auto.
+          left; congruence.
+        * exfalso; auto.
+      + xthd; try assumption.
+        red; red in H11.
+        destruct (orqs1@[pidx]) as [orq1|];
+          destruct (orqs2@[pidx]) as [orq2|]; simpl in *; auto;
+            try discriminate.
+        * destruct H11 as [rqi ?]; dest.
+          destruct H11; [|congruence].
+          eexists; split.
+          { left; rewrite <-H4; eassumption. }
+          { assumption. }
+        * destruct H11 as [rqi ?]; dest.
+          destruct H11; [congruence|].
+          subst; rewrite H11 in H1; inv H1.
+          auto.
+  Qed.
+
+  Lemma upLockedInv_orqs_preserved_rs_rq:
+    forall (orqs1 orqs2: ORqs Msg) msgs oidx pidx rqiu rqid,
+      UpLockedInv orqs1 msgs oidx ->
+      parentIdxOf dtr oidx = Some pidx ->
+      orqs1@[pidx] >>= (fun orq1 => orq1@[upRq]) = Some rqiu ->
+      orqs2@[pidx] >>= (fun orq2 => orq2@[upRq]) = None ->
+      orqs1@[pidx] >>= (fun orq1 => orq1@[downRq]) = None ->
+      orqs2@[pidx] >>= (fun orq2 => orq2@[downRq]) = Some rqid ->
+      rqiu.(rqi_midx_rsb) = rqid.(rqi_midx_rsb) ->
+      UpLockedInv orqs2 msgs oidx.
+  Proof.
+    unfold UpLockedInv; intros.
+    destruct H as [rqUp [down [pidx' ?]]]; dest.
+    rewrite H7 in H0; inv H0.
+    exists rqUp, down, pidx; repeat split; try assumption.
+    - red in H10; red.
+      destruct (orqs1@[pidx]) as [orq1|];
+        destruct (orqs2@[pidx]) as [orq2|]; simpl in *;
+          auto; try discriminate.
+      rewrite H2; auto.
+    - destruct H11.
+      + xfst; try assumption.
+        intro Hx; elim H12; clear H12.
+        red in Hx; red.
+        destruct (orqs1@[pidx]) as [orq1|];
+          destruct (orqs2@[pidx]) as [orq2|]; simpl in *; auto;
+            try discriminate.
+        destruct Hx as [rqi ?]; dest.
+        destruct H12; [congruence|].
+        exists rqiu; split; auto.
+        congruence.
+      + xsnd; try assumption.
+        intro Hx; elim H12; clear H12.
+        red in Hx; red.
+        destruct (orqs1@[pidx]) as [orq1|];
+          destruct (orqs2@[pidx]) as [orq2|]; simpl in *; auto;
+            try discriminate.
+        destruct Hx as [rqi ?]; dest.
+        destruct H12; [congruence|].
+        exists rqiu; split; auto.
+        congruence.
+      + xthd; try assumption.
+        red; red in H12.
+        destruct (orqs1@[pidx]) as [orq1|];
+          destruct (orqs2@[pidx]) as [orq2|]; simpl in *; auto;
+            try discriminate.
+        destruct H12 as [rqi ?]; dest.
+        destruct H12; [|congruence].
+        eexists; split.
+        { right; eassumption. }
+        { congruence. }
+  Qed.
+  
+  Corollary upLockedInv_orqs_preserved_non_parent_update:
+    forall orqs msgs oidx1 oidx2 orq,
+      UpLockedInv orqs msgs oidx1 ->
+      parentIdxOf dtr oidx1 <> Some oidx2 ->
+      UpLockedInv (orqs+[oidx2 <- orq]) msgs oidx1.
+  Proof.
+    intros.
+    destruct Hsd.
+    pose proof H.
+    destruct H3 as [rqUp [down [pidx ?]]]; dest.
+    eapply upLockedInv_orqs_preserved_parent_eq; eauto.
+    mred.
+  Qed.
+
+  Lemma upLockFreeInv_orqs_preserved_parent_eq:
+    forall (orqs1 orqs2: ORqs Msg) msgs oidx pidx,
+      UpLockFreeInv orqs1 msgs oidx ->
+      parentIdxOf dtr oidx = Some pidx ->
+      orqs1@[pidx] = orqs2@[pidx] ->
+      UpLockFreeInv orqs2 msgs oidx.
+  Proof.
+    unfold UpLockFreeInv; intros; dest.
+    destruct H; [left; assumption|right].
+    destruct H as [rqUp [down [pidx' ?]]]; dest.
+    rewrite H3 in H0; inv H0.
+    exists rqUp, down, pidx.
+    repeat split; try assumption.
+    unfold ONoLockTo in *.
+    rewrite <-H1; assumption.
+  Qed.
+
+  Lemma upLockFreeInv_orqs_preserved_self_update:
+    forall orqs msgs oidx orq,
+      UpLockFreeInv orqs msgs oidx ->
+      UpLockFreeInv (orqs+[oidx <- orq]) msgs oidx.
+  Proof.
+    unfold UpLockFreeInv; intros; dest.
+    destruct H; [left; assumption|right].
+    destruct H as [rqUp [down [pidx ?]]]; dest.
+    exists rqUp, down, pidx.
+    repeat split; try assumption.
+    red in H4; red.
+    apply parentIdxOf_not_eq in H1; [|destruct Hsd; assumption].
+    mred.
+  Qed.
+
+  Lemma upLockFreeInv_orqs_preserved_parent_some_up:
+    forall (orqs1 orqs2: ORqs Msg) msgs oidx pidx rqiu,
+      UpLockFreeInv orqs1 msgs oidx ->
+      parentIdxOf dtr oidx = Some pidx ->
+      orqs1@[pidx] >>= (fun orq1 => orq1@[upRq]) = None ->
+      orqs2@[pidx] >>= (fun orq2 => orq2@[upRq]) = Some rqiu ->
+      edgeDownTo dtr oidx <> Some (rqiu.(rqi_midx_rsb)) ->
+      orqs1@[pidx] >>= (fun orq1 => orq1@[downRq]) =
+      orqs2@[pidx] >>= (fun orq2 => orq2@[downRq]) ->
+      UpLockFreeInv orqs2 msgs oidx.
+  Proof.
+    unfold UpLockFreeInv; intros; dest.
+    destruct H; [left; assumption|right].
+    destruct H as [rqUp [down [pidx' ?]]]; dest.
+    exists rqUp, down, pidx.
+    repeat split; try assumption.
+    red.
+    destruct (orqs2@[pidx]) as [orq2|]; simpl in *; auto.
+    split.
+    - rewrite H2.
+      intro Hx; subst; congruence.
+    - rewrite H6 in H0; inv H0.
+      red in H9.
+      destruct (orqs1@[pidx]) as [orq1|]; simpl in *; dest.
+      + rewrite <-H4; assumption.
+      + rewrite <-H4; auto.
+  Qed.
+
+  Lemma upLockFreeInv_orqs_preserved_parent_some_down:
+    forall (orqs1 orqs2: ORqs Msg) msgs oidx pidx rqiu,
+      UpLockFreeInv orqs1 msgs oidx ->
+      parentIdxOf dtr oidx = Some pidx ->
+      orqs1@[pidx] >>= (fun orq1 => orq1@[downRq]) = None ->
+      orqs2@[pidx] >>= (fun orq2 => orq2@[downRq]) = Some rqiu ->
+      edgeDownTo dtr oidx <> Some (rqiu.(rqi_midx_rsb)) ->
+      orqs1@[pidx] >>= (fun orq1 => orq1@[upRq]) =
+      orqs2@[pidx] >>= (fun orq2 => orq2@[upRq]) ->
+      UpLockFreeInv orqs2 msgs oidx.
+  Proof.
+    unfold UpLockFreeInv; intros; dest.
+    destruct H; [left; assumption|right].
+    destruct H as [rqUp [down [pidx' ?]]]; dest.
+    exists rqUp, down, pidx.
+    repeat split; try assumption.
+    red.
+    destruct (orqs2@[pidx]) as [orq2|]; simpl in *; auto.
+    split.
+    - rewrite H6 in H0; inv H0.
+      red in H9.
+      destruct (orqs1@[pidx]) as [orq1|]; simpl in *; dest.
+      + rewrite <-H4; assumption.
+      + rewrite <-H4; auto.
+    - rewrite H2.
+      intro Hx; subst; congruence.
+  Qed.
+
+  Lemma upLockFreeInv_orqs_preserved_parent_none_up:
+    forall (orqs1 orqs2: ORqs Msg) msgs oidx pidx,
+      UpLockFreeInv orqs1 msgs oidx ->
+      parentIdxOf dtr oidx = Some pidx ->
+      orqs2@[pidx] >>= (fun orq2 => orq2@[upRq]) = None ->
+      orqs1@[pidx] >>= (fun orq1 => orq1@[downRq]) =
+      orqs2@[pidx] >>= (fun orq2 => orq2@[downRq]) ->
+      UpLockFreeInv orqs2 msgs oidx.
+  Proof.
+    unfold UpLockFreeInv; intros; dest.
+    destruct H; [left; assumption|right].
+    destruct H as [rqUp [down [pidx' ?]]]; dest.
+    rewrite H4 in H0; inv H0.
+    exists rqUp, down, pidx.
+    repeat split; try assumption.
+    red; red in H7; dest.
+    destruct (orqs2@[pidx]) as [orq2|]; simpl in *; auto.
+    split.
+    - rewrite H1; auto.
+    - destruct (orqs1@[pidx]) as [orq1|]; simpl in *; dest.
+      + rewrite <-H2; assumption.
+      + rewrite <-H2; auto.
+  Qed.
+
+  Lemma upLockFreeInv_orqs_preserved_parent_none_down:
+    forall (orqs1 orqs2: ORqs Msg) msgs oidx pidx,
+      UpLockFreeInv orqs1 msgs oidx ->
+      parentIdxOf dtr oidx = Some pidx ->
+      orqs2@[pidx] >>= (fun orq2 => orq2@[downRq]) = None ->
+      orqs1@[pidx] >>= (fun orq1 => orq1@[upRq]) =
+      orqs2@[pidx] >>= (fun orq2 => orq2@[upRq]) ->
+      UpLockFreeInv orqs2 msgs oidx.
+  Proof.
+    unfold UpLockFreeInv; intros; dest.
+    destruct H; [left; assumption|right].
+    destruct H as [rqUp [down [pidx' ?]]]; dest.
+    rewrite H4 in H0; inv H0.
+    exists rqUp, down, pidx.
+    repeat split; try assumption.
+    red; red in H7.
+    destruct (orqs2@[pidx]) as [orq2|]; simpl in *; auto.
+    split.
+    - destruct (orqs1@[pidx]) as [orq1|]; simpl in *; dest.
+      + rewrite <-H2; assumption.
+      + rewrite <-H2; auto.
+    - rewrite H1; auto.
+  Qed.
+
+  Lemma upLockFreeInv_orqs_preserved_rs_rq:
+    forall (orqs1 orqs2: ORqs Msg) msgs oidx pidx rqiu rqid,
+      UpLockFreeInv orqs1 msgs oidx ->
+      parentIdxOf dtr oidx = Some pidx ->
+      orqs1@[pidx] >>= (fun orq1 => orq1@[upRq]) = Some rqiu ->
+      orqs2@[pidx] >>= (fun orq2 => orq2@[upRq]) = None ->
+      orqs1@[pidx] >>= (fun orq1 => orq1@[downRq]) = None ->
+      orqs2@[pidx] >>= (fun orq2 => orq2@[downRq]) = Some rqid ->
+      rqiu.(rqi_midx_rsb) = rqid.(rqi_midx_rsb) ->
+      UpLockFreeInv orqs2 msgs oidx.
+  Proof.
+    unfold UpLockFreeInv; intros; dest.
+    destruct H; [left; assumption|right].
+    destruct H as [rqUp [down [pidx' ?]]]; dest.
+    rewrite H7 in H0; inv H0.
+    exists rqUp, down, pidx.
+    repeat split; try assumption.
+    red; red in H10.
+    destruct (orqs2@[pidx]) as [orq2|]; simpl in *; auto.
+    split.
+    - rewrite H2; auto.
+    - rewrite H4.
+      destruct (orqs1@[pidx]) as [orq1|]; simpl in *; dest.
+      + rewrite H1 in H0; congruence.
+      + discriminate.
+  Qed.
+
+  Corollary upLockFreeInv_orqs_preserved_non_parent_update:
+    forall orqs msgs oidx1 oidx2 orq,
+      UpLockFreeInv orqs msgs oidx1 ->
+      parentIdxOf dtr oidx1 <> Some oidx2 ->
+      UpLockFreeInv (orqs+[oidx2 <- orq]) msgs oidx1.
+  Proof.
+    intros.
+    destruct Hsd.
+    pose proof H.
+    destruct H3; [left; assumption|].
+    destruct H3 as [rqUp [down [pidx ?]]]; dest.
+    eapply upLockFreeInv_orqs_preserved_parent_eq; eauto.
+    mred.
+  Qed.
+
+  Lemma upLockInv_step_ext_in:
+    forall oss orqs msgs eins,
+      UpLockInv {| bst_oss := oss; bst_orqs := orqs; bst_msgs := msgs |} ->
+      eins <> nil ->
+      ValidMsgsExtIn sys eins ->
+      UpLockInv {| bst_oss := oss;
+                   bst_orqs := orqs;
+                   bst_msgs := enqMsgs eins msgs |}.
+  Proof.
+    unfold UpLockInv; simpl; intros.
+    red; intros.
+    specialize (H oidx H2).
+
+    destruct H1.
+    assert (DisjList (idsOf eins) (sys_minds sys)).
+    { eapply DisjList_SubList; eauto.
+      apply DisjList_comm.
+      apply sys_minds_sys_merqs_DisjList.
+    }
+    
+    destruct (orqs@[oidx]) as [orq|]; simpl in *; dest.
+    - red in H; red.
+      remember (orq@[upRq]) as orqi.
+      destruct orqi as [rqi|].
+      + apply upLockedInv_disj_enqMsgs_preserved; assumption.
+      + apply upLockFreeInv_disj_enqMsgs_preserved; assumption.
+    - red in H; simpl in H.
+      red in H3; simpl in H3.
+      red; simpl.
+      apply upLockFreeInv_disj_enqMsgs_preserved; assumption.
+  Qed.
+
+  Lemma upLockInv_step_ext_out:
+    forall oss orqs msgs eouts,
+      UpLockInv {| bst_oss := oss; bst_orqs := orqs; bst_msgs := msgs |} ->
+      eouts <> nil ->
+      Forall (FirstMPI msgs) eouts ->
+      ValidMsgsExtOut sys eouts ->
+      UpLockInv {| bst_oss := oss;
+                   bst_orqs := orqs;
+                   bst_msgs := deqMsgs (idsOf eouts) msgs |}.
+  Proof.
+    unfold UpLockInv; simpl; intros.
+    red; intros.
+    specialize (H oidx H3).
+
+    destruct H2.
+    assert (DisjList (idsOf eouts) (sys_minds sys)).
+    { eapply DisjList_SubList; eauto.
+      apply DisjList_comm.
+      apply sys_minds_sys_merss_DisjList.
+    }
+    
+    destruct (orqs@[oidx]) as [orq|]; simpl in *; dest.
+    - red in H; red.
+      remember (orq@[upRq]) as orqi.
+      destruct orqi as [rqi|].
+      + apply upLockedInv_disj_deqMsgs_preserved; assumption.
+      + apply upLockFreeInv_disj_deqMsgs_preserved; assumption.
+    - red in H; simpl in H.
+      red in H4; simpl in H4.
+      red; simpl.
+      apply upLockFreeInv_disj_deqMsgs_preserved; assumption.
+  Qed.
+
+  Section InternalStep.
+    Variables (oss: OStates oifc) (orqs: ORqs Msg) (msgs: MessagePool Msg)
+              (obj: Object oifc) (rule: Rule oifc)
+              (post: OState oifc) (porq: ORq Msg) (mins: list (Id Msg))
+              (nost: OState oifc) (norq: ORq Msg) (mouts: list (Id Msg)).
+
+    Hypotheses
+      (Hfpok: FootprintsOk
+                dtr sys {| bst_oss := oss; bst_orqs := orqs; bst_msgs := msgs |})
+      (HobjIn: In obj (sys_objs sys))
+      (HruleIn: In rule (obj_rules obj))
+      (Hporq: orqs@[obj_idx obj] = Some porq)
+      (Hpost: oss@[obj_idx obj] = Some post)
+      (HminsF: Forall (FirstMPI msgs) mins)
+      (HminsV: ValidMsgsIn sys mins)
+      (Hprec: rule_precond rule post porq mins)
+      (Htrs: rule_trs rule post porq mins = (nost, norq, mouts))
+      (HmoutsV: ValidMsgsOut sys mouts)
+      (Hmdisj: DisjList (idsOf mins) (idsOf mouts)).
+
+    Lemma deqMP_rq_filter_rs_eq:
+      forall midx msg,
+        msg_type msg = MRq ->
+        FirstMPI msgs (midx, msg) ->
+        filter (fun msg => msg_type msg ==n MRs)
+               (findQ midx msgs) =
+        filter (fun msg => msg_type msg ==n MRs)
+               (findQ midx (deqMP midx msgs)).
+    Proof.
+      intros.
+      unfold FirstMPI, FirstMP, firstMP in H0.
+      unfold deqMP, idOf in *; simpl in *.
+      destruct (findQ midx msgs); [discriminate|].
+      simpl in H0; inv H0.
+      unfold findQ; mred; simpl.
+      rewrite H; simpl.
+      reflexivity.
+    Qed.
+
+    Lemma deqMP_rs_filter_rq_eq:
+      forall midx msg,
+        msg_type msg = MRs ->
+        FirstMPI msgs (midx, msg) ->
+        filter (fun msg => msg_type msg ==n MRq)
+               (findQ midx msgs) =
+        filter (fun msg => msg_type msg ==n MRq)
+               (findQ midx (deqMP midx msgs)).
+    Proof.
+      intros.
+      unfold FirstMPI, FirstMP, firstMP in H0.
+      unfold deqMP, idOf in *; simpl in *.
+      destruct (findQ midx msgs); [discriminate|].
+      simpl in H0; inv H0.
+      unfold findQ; mred; simpl.
+      rewrite H; simpl.
+      reflexivity.
+    Qed.
+
+    Ltac disc_rule_custom ::=
+      match goal with
+      | [H: FootprintUpOkEx _ _ _ /\ _ |- _] => destruct H
+      | [H: _ /\ FootprintDownOkEx _ _ _ _ |- _] => destruct H
+      | [H: FootprintUpOkEx _ _ _ |- _] =>
+        let rqFrom := fresh "rqFrom" in
+        let rqTo := fresh "rqTo" in
+        let rsFrom := fresh "rsFrom" in
+        let rsbTo := fresh "rsbTo" in
+        destruct H as [rqFrom [rqTo [rsFrom [rsbTo ?]]]]; dest
+      | [H: FootprintUpOk _ _ _ _ _ _ |- _] =>
+        let cidx := fresh "cidx" in
+        destruct H as [cidx ?]; dest
+
+      | [H: FootprintDownOkEx _ _ _ _ |- _] =>
+        let rqFrom := fresh "rqFrom" in
+        let rqTos := fresh "rqTos" in
+        let rssFrom := fresh "rssFrom" in
+        let rsbTo := fresh "rsbTo" in
+        destruct H as [rqFrom [rqTos [rssFrom [rsbTo ?]]]]; dest
+      | [H: FootprintUpDownOk _ _ _ _ _ _ _ \/
+            FootprintDownDownOk _ _ _ _ _ _ |- _] => destruct H
+      | [H: exists _, FootprintUpDownOk _ _ _ _ _ _ _ |- _] =>
+        let rqFrom := fresh "rqFrom" in
+        destruct H as [rqFrom ?]
+      | [H: FootprintUpDownOk _ _ _ _ _ _ _ |- _] =>
+        let upCIdx := fresh "upCIdx" in
+        let upCObj := fresh "upCObj" in
+        destruct H as [upCIdx [upCObj ?]]; dest
+      | [H: FootprintDownDownOk _ _ _ _ _ _ |- _] => red in H; dest
+      end.
+
+    Lemma upLockInvORq_step_int_me:
+      UpLockInvORq orqs msgs (obj_idx obj) porq ->
+      In (obj_idx obj) (map (@obj_idx _) (sys_objs sys)) ->
+      GoodRqRsRule dtr sys (obj_idx obj) rule ->
+      UpLockInvORq (orqs+[obj_idx obj <- norq])
+                   (enqMsgs mouts (deqMsgs (idsOf mins) msgs))
+                   (obj_idx obj) norq.
+    Proof.
+      intros.
+      destruct Hsd.
+      red in H; red.
+      good_rqrs_rule_cases rule.
+
+      - (** case [ImmDownRule] *)
+        disc_rule_conds.
+        apply upLockFreeInv_orqs_preserved_self_update.
+        eapply upLockFreeInv_msgs_preserved; eauto.
+        + remember (rqEdgeUpFrom dtr (obj_idx obj)) as orqUp.
+          destruct orqUp as [rqUp|]; auto.
+          solve_q.
+        + remember (edgeDownTo dtr (obj_idx obj)) as odown.
+          destruct odown as [down|]; auto.
+          solve_q.
+
+      - (** case [ImmUpRule] *)
+        disc_rule_conds.
+        destruct (norq@[upRq]).
+        + apply upLockedInv_orqs_preserved_self_update.
+          eapply upLockedInv_msgs_preserved; eauto.
+          * destruct H as [rqUp [down [pidx ?]]]; dest.
+            disc_rule_conds.
+            solve_q.
+          * disc_rule_conds.
+            solve_q.
+            eapply deqMP_rq_filter_rs_eq; eauto.
+        + apply upLockFreeInv_orqs_preserved_self_update.
+          eapply upLockFreeInv_msgs_preserved; eauto.
+          * remember (rqEdgeUpFrom dtr (obj_idx obj)) as orqUp.
+            destruct orqUp as [rqUp|]; auto.
+            solve_q.
+          * disc_rule_conds.
+            solve_q.
+            eapply deqMP_rq_filter_rs_eq; eauto.
+
+      - (** case [RqFwdRule] *)
+        disc_rule_conds.
+        + (** case [RqUpUp]; setting an uplock. *)
+          apply upLockedInv_orqs_preserved_self_update.
+          red in H.
+          pose proof (rqEdgeUpFrom_Some Hsd _ H5).
+          destruct H10 as [rsUp [down [pidx ?]]]; dest.
+          disc_rule_conds.
+          destruct H; [discriminate|].
+          destruct H as [rqUp [down' [pidx' ?]]]; dest.
+          disc_rule_conds.
+          do 3 eexists; repeat split; try eassumption.
+          * solve_q.
+            rewrite H19; simpl; omega.
+          * solve_q.
+            unfold rssQ in H20; rewrite H20.
+            simpl; omega.
+          * apply ONoLockTo_ONoSameLockTo; assumption.
+          * xfst.
+            { solve_q.
+              rewrite H19; reflexivity.
+            }
+            { solve_q.
+              unfold rssQ in H20; rewrite H20; auto.
+            }
+            { apply ONoLockTo_not_OLockedTo; assumption. }
+
+        + (** case [RqUpDown]; setting a downlock. *)
+          remember (porq@[upRq]) as orqiu; destruct orqiu as [rqiu|].
+          * apply upLockedInv_orqs_preserved_self_update.
+            apply upLockedInv_msgs_preserved with (msgs1:= msgs);
+              [assumption| |].
+            { destruct H as [rqUp [down [pidx ?]]]; dest.
+              rewrite H.
+              solve_q.
+            }
+            { destruct H as [rqUp [down [pidx ?]]]; dest.
+              disc_rule_conds.
+              solve_q.
+            }
+
+          * apply upLockFreeInv_orqs_preserved_self_update.
+            apply upLockFreeInv_msgs_preserved with (msgs1:= msgs);
+              [assumption| |].
+            { destruct H.
+              { remember (rqEdgeUpFrom dtr (obj_idx obj)) as orqUp.
+                destruct orqUp; auto.
+                eapply eq_sym, rqEdgeUpFrom_Some in HeqorqUp; [|eassumption].
+                dest; disc_rule_conds.
+              }
+              { destruct H as [rqUp [down [pidx ?]]]; dest.
+                disc_rule_conds.
+                solve_q.
+              }
+            }
+            { destruct H.
+              { remember (edgeDownTo dtr (obj_idx obj)) as odown.
+                destruct odown; auto.
+                eapply eq_sym, edgeDownTo_Some in Heqodown; [|eassumption].
+                dest; disc_rule_conds.
+              }
+              { destruct H as [rqUp [down [pidx ?]]]; dest.
+                disc_rule_conds.
+                solve_q.
+              }
+            }
+
+        + (** case [RqDownDown]; setting a downlock *)
+          remember (porq@[upRq]) as orqiu; destruct orqiu as [rqiu|].
+          * apply upLockedInv_orqs_preserved_self_update.
+            apply upLockedInv_msgs_preserved with (msgs1:= msgs);
+              [assumption| |].
+            { red in H; destruct H as [rqUp [down [pidx ?]]]; dest.
+              disc_rule_conds.
+              solve_q.
+            }
+            { red in H; destruct H as [rqUp [down [pidx ?]]]; dest.
+              disc_rule_conds.
+              solve_q.
+              eapply deqMP_rq_filter_rs_eq; eauto.
+            }
+
+          * apply upLockFreeInv_orqs_preserved_self_update.
+            apply upLockFreeInv_msgs_preserved with (msgs1:= msgs);
+              [assumption| |].
+            { destruct H.
+              { remember (rqEdgeUpFrom dtr (obj_idx obj)) as orqUp.
+                destruct orqUp; auto.
+                eapply eq_sym, rqEdgeUpFrom_Some in HeqorqUp; [|eassumption].
+                dest; disc_rule_conds.
+              }
+              { destruct H as [rqUp [down [pidx ?]]]; dest.
+                disc_rule_conds.
+                solve_q.
+              }
+            }
+            { destruct H.
+              { remember (edgeDownTo dtr (obj_idx obj)) as odown.
+                destruct odown; auto.
+                eapply eq_sym, edgeDownTo_Some in Heqodown; [|eassumption].
+                dest; disc_rule_conds.
+              }
+              { destruct H as [rqUp [down [pidx ?]]]; dest.
+                disc_rule_conds.
+                solve_q.
+                eapply deqMP_rq_filter_rs_eq; eauto.
+              }
+            }
+
+      - (** case [RsBackRule] *)
+        good_footprint_get (obj_idx obj).
+        disc_rule_conds.
+        + (** case [FootprintReleasingUp]; releasing the uplock. *)
+          apply upLockFreeInv_orqs_preserved_self_update.
+          destruct i as [rsDown rsbm]; simpl in *.
+          destruct H as [rqUp [down [pidx ?]]]; dest.
+          disc_rule_conds.
+          eapply xor3_inv_2 with (B:= length (rssQ msgs rsDown) = 1) in H20;
+            [dest|eapply rssQ_length_one; eauto].
+          remember (rqi_midx_rsb rqi) as rsbTo; clear HeqrsbTo.
+          right.
+          exists rqTo, rsDown, pidx.
+          repeat split; try assumption.
+          * solve_q.
+            apply length_zero_iff_nil; omega.
+          * solve_q.
+            apply findQ_In_deqMP_FirstMP in H9; simpl in H9.
+            unfold rssQ in H18; rewrite <-H9 in H18.
+            simpl in H18; rewrite H12 in H18; simpl in H18.
+            apply length_zero_iff_nil; omega.
+          * apply not_ONoLockTo_OLockedTo; auto.
+          
+        + (** case [FootprintReleasingDown]-1 *)
+          remember (porq@[upRq]) as orqiu; destruct orqiu as [rqiu|].
+          * apply upLockedInv_orqs_preserved_self_update.
+            apply upLockedInv_msgs_preserved with (msgs1:= msgs);
+              [assumption| |].
+            { destruct H as [rqUp [down [pidx ?]]]; dest.
+              disc_rule_conds.
+              rewrite H17.
+              solve_q.
+            }
+            { destruct H as [rqUp [down [pidx ?]]]; dest.
+              disc_rule_conds.
+              rewrite H17.
+              solve_q.
+            }              
+          * apply upLockFreeInv_orqs_preserved_self_update.
+            apply upLockFreeInv_msgs_preserved with (msgs1:= msgs);
+              [assumption| |].
+            { destruct H.
+              { remember (rqEdgeUpFrom dtr (obj_idx obj)) as orqUp.
+                destruct orqUp; auto.
+                eapply eq_sym, rqEdgeUpFrom_Some in HeqorqUp; [|eassumption].
+                dest; disc_rule_conds.
+              }
+              { destruct H as [rqUp [down [pidx ?]]]; dest.
+                disc_rule_conds.
+                rewrite H17.
+                solve_q.
+              }
+            }
+            { destruct H.
+              { remember (edgeDownTo dtr (obj_idx obj)) as odown.
+                destruct odown; auto.
+                eapply eq_sym, edgeDownTo_Some in Heqodown; [|eassumption].
+                dest; disc_rule_conds.
+              }
+              { destruct H as [rqUp [down [pidx ?]]]; dest.
+                disc_rule_conds.
+                rewrite H17.
+                solve_q.
+              }
+            }
+
+        + (** case [FootprintReleasingDown]-2 *)
+          remember (porq@[upRq]) as orqiu; destruct orqiu as [rqiu|].
+          * apply upLockedInv_orqs_preserved_self_update.
+            apply upLockedInv_msgs_preserved with (msgs1:= msgs);
+              [assumption| |].
+            { destruct H as [rqUp [down [pidx ?]]]; dest.
+              disc_rule_conds.
+              rewrite H17.
+              solve_q.
+            }
+            { destruct H as [rqUp [down [pidx ?]]]; dest.
+              disc_rule_conds.
+              rewrite H17.
+              solve_q.
+            }
+          * apply upLockFreeInv_orqs_preserved_self_update.
+            apply upLockFreeInv_msgs_preserved with (msgs1:= msgs);
+              [assumption| |].
+            { destruct H.
+              { remember (rqEdgeUpFrom dtr (obj_idx obj)) as orqUp.
+                destruct orqUp; auto.
+                eapply eq_sym, rqEdgeUpFrom_Some in HeqorqUp; [|eassumption].
+                dest; disc_rule_conds.
+              }
+              { destruct H as [rqUp [down [pidx ?]]]; dest.
+                disc_rule_conds.
+                rewrite H17.
+                solve_q.
+              }
+            }
+            { destruct H.
+              { remember (edgeDownTo dtr (obj_idx obj)) as odown.
+                destruct odown; auto.
+                eapply eq_sym, edgeDownTo_Some in Heqodown; [|eassumption].
+                dest; disc_rule_conds.
+              }
+              { destruct H as [rqUp [down [pidx ?]]]; dest.
+                disc_rule_conds.
+                rewrite H17.
+                solve_q.
+              } 
+            }
+
+      - (** case [RsDownRqDownRule] *)
+        disc_rule_conds.
+        apply upLockFreeInv_orqs_preserved_self_update.
+        destruct H as [rqUp [down [pidx ?]]]; dest.
+        disc_rule_conds.
+        eapply xor3_inv_2 with (B:= length (rssQ msgs rsFrom) = 1) in H17;
+          [dest|eapply rssQ_length_one; eauto].
+        red; right.
+        exists rqUp, rsFrom, pidx; repeat split; try assumption.
+        + solve_q.
+          apply length_zero_iff_nil; omega.
+        + solve_q.
+          apply findQ_In_deqMP_FirstMP in H7; simpl in H7.
+          unfold rssQ in H14; rewrite <-H7 in H14.
+          simpl in H14; rewrite H5 in H14; simpl in H14.
+          apply length_zero_iff_nil; omega.
+        + apply not_ONoLockTo_OLockedTo; auto.
+    Qed.
+
+    Lemma upLockInvORq_step_int_parent:
+      forall oidx,
+        UpLockInvORq orqs msgs oidx ((orqs@[oidx]) >>=[[]] (fun orq => orq)) ->
+        In oidx (map (@obj_idx _) (sys_objs sys)) ->
+        GoodRqRsRule dtr sys (obj_idx obj) rule ->
+        parentIdxOf dtr oidx = Some (obj_idx obj) ->
+        UpLockInvORq (orqs+[obj_idx obj <- norq])
+                     (enqMsgs mouts (deqMsgs (idsOf mins) msgs)) oidx
+                     ((orqs@[ oidx]) >>=[[]] (fun orq => orq)).
+    Proof.
+      intros.
+      destruct Hsd.
+      red in H; red.
+      good_rqrs_rule_cases rule.
+
+      - (** case [ImmDownRule] *)
+        find_if_inside.
+        + eapply upLockedInv_orqs_preserved_parent_eq with (orqs1:= orqs).
+          * disc_rule_conds.
+            destruct (eq_nat_dec cidx oidx); subst.
+            { destruct H as [rqUp [down [pidx ?]]]; dest.
+              exists rqUp, down, pidx.
+              disc_rule_conds.
+
+              assert (length (rssQ (enqMP rsTo rsm (deqMP rqFrom msgs)) rsTo) = 1).
+              { solve_q.
+                rewrite filter_app; simpl.
+                rewrite H6; simpl.
+                rewrite app_length; simpl.
+                eapply xor3_inv_1
+                  with (A:= length (findQ rqFrom msgs) = 1) in H14; dest.
+                { unfold rssQ in H2, H9; omega. }
+                { eapply findQ_length_one; eauto. }
+              }
+              rewrite H2; clear H2.
+
+              solve_q.
+              repeat split; try assumption.
+              { apply findQ_In_deqMP_FirstMP in H11; simpl in H11.
+                rewrite <-H11 in H7; simpl in H7.
+                omega.
+              }
+              { omega. }
+              { xsnd.
+                { apply findQ_In_deqMP_FirstMP in H11; simpl in H11.
+                  rewrite <-H11 in H7; simpl in H7.
+                  omega.
+                }
+                { reflexivity. }
+                { apply ONoLockTo_not_OLockedTo.
+                  red; disc_rule_conds; auto.
+                }
+              }
+            }
+            { eapply parentIdxOf_Some in H2; [|eassumption].
+              destruct H2 as [rqUp [rsUp [down ?]]]; dest.
+              eapply upLockedInv_msgs_preserved; [eassumption| |].
+              { disc_rule_conds; solve_q. }
+              { disc_rule_conds; solve_q. }
+            }
+          * eassumption.
+          * disc_rule_conds.
+          
+        + eapply upLockFreeInv_orqs_preserved_parent_eq with (orqs1:= orqs).
+          * disc_rule_conds.
+            destruct (eq_nat_dec cidx oidx); subst.
+            { exfalso.
+              destruct H; [congruence|].
+              destruct H as [rqUp [down [pidx ?]]]; dest.
+              disc_rule_conds.
+              apply FirstMP_InMP in H11.
+              red in H11; simpl in H11; rewrite H7 in H11.
+              elim H11.
+            }
+            { destruct H; [left; assumption|right].
+              destruct H as [rqUp [down [pidx ?]]]; dest.
+              exists rqUp, down, pidx.
+              repeat split; try assumption.
+              { solve_q; assumption. }
+              { solve_q; assumption. }
+            }
+          * eassumption.
+          * disc_rule_conds.
+
+      - (** case [ImmUpRule] *)
+        find_if_inside.
+        + disc_rule_conds.
+          eapply upLockedInv_orqs_preserved_parent_eq with (orqs1:= orqs);
+            [|eassumption|mred].
+          apply upLockedInv_msgs_preserved with (msgs1:= msgs);
+            [assumption| |].
+          * destruct H as [rqUp [down [pidx ?]]]; dest.
+            disc_rule_conds.
+            solve_q.
+          * destruct H as [rqUp [down [pidx ?]]]; dest.
+            disc_rule_conds.
+            solve_q.
+        + disc_rule_conds.
+          eapply upLockFreeInv_orqs_preserved_parent_eq with (orqs1:= orqs);
+            [|eassumption|mred].
+          apply upLockFreeInv_msgs_preserved with (msgs1:= msgs);
+            [assumption| |].
+          * destruct H.
+            { remember (rqEdgeUpFrom dtr oidx) as orqUp.
+              destruct orqUp; auto.
+              eapply eq_sym, rqEdgeUpFrom_Some in HeqorqUp; [|eassumption].
+              dest; disc_rule_conds.
+            }
+            { destruct H as [rqUp [down [pidx ?]]]; dest.
+              disc_rule_conds.
+              solve_q.
+            }
+          * destruct H.
+            { remember (edgeDownTo dtr oidx) as odown.
+              destruct odown; auto.
+              eapply eq_sym, edgeDownTo_Some in Heqodown; [|eassumption].
+              dest; disc_rule_conds.
+            }
+            { destruct H as [rqUp [down [pidx ?]]]; dest.
+              disc_rule_conds.
+              solve_q.
+            }
+
+      - (** case [RqFwdRule] *)
+        disc_rule_conds.
+        + (** case [RqUpUp] *)
+          destruct (eq_nat_dec cidx oidx); subst.
+          * find_if_inside.
+            { destruct H as [rqUp [down [pidx ?]]]; dest.
+              exists rqUp, down, pidx.
+              disc_rule_conds.
+
+              apply xor3_inv_1
+                with (A:= length (findQ rqFrom msgs) = 1) in H21;
+                [dest|eapply findQ_length_one; eauto].
+
+              assert (length (findQ rqFrom (enqMP rqTo rqtm (deqMP rqFrom msgs))) = 0).
+              { solve_q.
+                apply findQ_In_deqMP_FirstMP in H14; simpl in H14.
+                rewrite <-H14 in H16; simpl in H16.
+                omega.
+              }
+              rewrite H5; clear H5.
+
+              assert (length (rssQ (enqMP rqTo rqtm (deqMP rqFrom msgs))
+                                   (rqi_midx_rsb rqi)) = 0).
+              { solve_q.
+                unfold rssQ in H1, H19; omega.
+              }
+              rewrite H5; clear H5.
+
+              repeat split; try assumption; try omega.
+              { unfold ONoSameLockTo, OLockedTo in *.
+                mred; simpl; mred.
+                destruct (porq@[downRq]) as [rqid|]; auto.
+                right.
+                intro Hx; elim H2; eauto.
+              }
+              { xthd; try discriminate.
+                red; mred; simpl; mred.
+                eexists; split; [left; reflexivity|reflexivity].
+              }
+            }
+            { destruct H; [left; assumption|right].
+              destruct H as [rqUp [down [pidx ?]]]; dest.
+              exfalso.
+              disc_rule_conds.
+              apply FirstMP_InMP in H14.
+              red in H14; simpl in H14; rewrite H16 in H14.
+              elim H14.
+            }
+          * find_if_inside.
+            { apply upLockedInv_orqs_preserved_parent_some_up
+                with (orqs1:= orqs) (pidx:= obj_idx obj) (rqiu:= rqi);
+                auto; try (repeat (mred; simpl); fail).
+              { eapply upLockedInv_msgs_preserved; [eassumption| |].
+                { destruct H as [rqUp [down [pidx ?]]]; dest.
+                  disc_rule_conds.
+                  solve_q.
+                }
+                { destruct H as [rqUp [down [pidx ?]]]; dest.
+                  disc_rule_conds.
+                  solve_q.
+                }
+              }
+              { intro Hx.
+                elim (rqrsDTree_down_down_not_eq Hsd n H9 Hx).
+                reflexivity.
+              }
+            }
+            { apply upLockFreeInv_orqs_preserved_parent_some_up
+                with (orqs1:= orqs) (pidx:= obj_idx obj) (rqiu:= rqi);
+                auto; try (repeat (mred; simpl); fail).
+              { eapply upLockFreeInv_msgs_preserved; [eassumption| |].
+                { destruct H.
+                  { remember (rqEdgeUpFrom dtr oidx) as orqUp.
+                    destruct orqUp; auto.
+                    eapply eq_sym, rqEdgeUpFrom_Some in HeqorqUp; [|eassumption].
+                    dest; disc_rule_conds.
+                  }
+                  { destruct H as [rqUp [down [pidx ?]]]; dest.
+                    disc_rule_conds.
+                    solve_q.
+                  }
+                }
+                { destruct H.
+                  { remember (edgeDownTo dtr oidx) as odown.
+                    destruct odown; auto.
+                    eapply eq_sym, edgeDownTo_Some in Heqodown; [|eassumption].
+                    dest; disc_rule_conds.
+                  }
+                  { destruct H as [rqUp [down [pidx ?]]]; dest.
+                    disc_rule_conds.
+                    solve_q.
+                  }
+                }
+              }
+              { intro Hx.
+                elim (rqrsDTree_down_down_not_eq Hsd n H9 Hx).
+                reflexivity.
+              }
+            }
+
+        + (** case [RqUpDown] *)
+          destruct (eq_nat_dec (obj_idx upCObj) oidx); subst.
+          * find_if_inside.
+            { destruct H as [rqUp [down [pidx ?]]]; dest.
+              exists rqUp, down, pidx.
+              disc_rule_conds.
+
+              apply xor3_inv_1
+                with (A:= length (findQ rqFrom msgs) = 1) in H20;
+                [dest|eapply findQ_length_one; eauto].
+
+              assert (length (findQ rqFrom (enqMsgs mouts (deqMP rqFrom msgs))) = 0).
+              { solve_q.
+                apply findQ_In_deqMP_FirstMP in H14; simpl in H14.
+                rewrite <-H14 in H16; simpl in H16.
+                omega.
+              }
+              rewrite H7; clear H7.
+
+              assert (length (rssQ (enqMsgs mouts (deqMP rqFrom msgs))
+                                   (rqi_midx_rsb rqi)) = 0).
+              { solve_q.
+                unfold rssQ in H2, H17; omega.
+              }
+              rewrite H7; clear H7.
+
+              repeat split; try assumption; try omega.
+              { unfold ONoSameLockTo, OLockedTo in *.
+                mred; simpl; mred.
+                destruct (porq@[upRq]) as [rqiu|]; auto.
+                left.
+                intro Hx; elim H6; eauto.
+              }
+              { xthd; try discriminate.
+                red; mred; simpl; mred.
+                eexists; split; [right; reflexivity|reflexivity].
+              }
+            }
+            { destruct H; [left; assumption|right].
+              destruct H as [rqUp [down [pidx ?]]]; dest.
+              exfalso.
+              disc_rule_conds.
+              apply FirstMP_InMP in H14.
+              red in H14; simpl in H14; rewrite H16 in H14.
+              elim H14.
+            }
+          * find_if_inside.
+            { apply upLockedInv_orqs_preserved_parent_some_down
+                with (orqs1:= orqs) (pidx:= obj_idx obj) (rqiu:= rqi);
+                auto; try (repeat (mred; simpl); fail).
+              { eapply upLockedInv_msgs_preserved; [eassumption| |].
+                { destruct H as [rqUp [down [pidx ?]]]; dest.
+                  disc_rule_conds.
+                  solve_q.
+                }
+                { destruct H as [rqUp [down [pidx ?]]]; dest.
+                  disc_rule_conds.
+                  rewrite rssQ_enqMsgs_rqs by assumption.
+                  solve_q.
+                }
+              }
+              { intro Hx.
+                elim (rqrsDTree_down_down_not_eq Hsd n H9 Hx).
+                reflexivity.
+              }
+            }
+            { apply upLockFreeInv_orqs_preserved_parent_some_down
+                with (orqs1:= orqs) (pidx:= obj_idx obj) (rqiu:= rqi);
+                auto; try (repeat (mred; simpl); fail).
+              { eapply upLockFreeInv_msgs_preserved; [eassumption| |].
+                { destruct H.
+                  { remember (rqEdgeUpFrom dtr oidx) as orqUp.
+                    destruct orqUp; auto.
+                    eapply eq_sym, rqEdgeUpFrom_Some in HeqorqUp; [|eassumption].
+                    dest; disc_rule_conds.
+                  }
+                  { destruct H as [rqUp [down [pidx ?]]]; dest.
+                    disc_rule_conds.
+                    solve_q.
+                  }
+                }
+                { destruct H.
+                  { remember (edgeDownTo dtr oidx) as odown.
+                    destruct odown; auto.
+                    eapply eq_sym, edgeDownTo_Some in Heqodown; [|eassumption].
+                    dest; disc_rule_conds.
+                  }
+                  { destruct H as [rqUp [down [pidx ?]]]; dest.
+                    disc_rule_conds.
+                    rewrite rssQ_enqMsgs_rqs by assumption.
+                    solve_q.
+                  }
+                }
+              }
+              { intro Hx.
+                elim (rqrsDTree_down_down_not_eq Hsd n H9 Hx).
+                reflexivity.
+              }
+            }
+
+        + (** case [RqDownDown] *)
+          find_if_inside.
+          * apply upLockedInv_orqs_preserved_parent_some_down
+              with (orqs1:= orqs) (pidx:= obj_idx obj) (rqiu:= rqi);
+              auto; try (repeat (mred; simpl); fail).
+            { apply upLockedInv_msgs_preserved with (msgs1:= msgs);
+                [assumption| |].
+              { destruct H as [rqUp [down [pidx ?]]]; dest.
+                disc_rule_conds.
+                solve_q.
+              }
+              { destruct H as [rqUp [down [pidx ?]]]; dest.
+                disc_rule_conds.
+                rewrite rssQ_enqMsgs_rqs by assumption.
+                solve_q.
+              }
+            }
+            { intro Hx.
+              elim (rqrsDTree_rsUp_down_not_eq Hsd _ _ H5 Hx).
+              reflexivity.
+            }
+          * apply upLockFreeInv_orqs_preserved_parent_some_down
+              with (orqs1:= orqs) (pidx:= obj_idx obj) (rqiu:= rqi);
+              auto; try (repeat (mred; simpl); fail).
+            { apply upLockFreeInv_msgs_preserved with (msgs1:= msgs);
+                [assumption| |].
+              { destruct H.
+                { remember (rqEdgeUpFrom dtr oidx) as orqUp.
+                  destruct orqUp; auto.
+                  eapply eq_sym, rqEdgeUpFrom_Some in HeqorqUp; [|eassumption].
+                  dest; disc_rule_conds.
+                }
+                { destruct H as [rqUp [down [pidx ?]]]; dest.
+                  disc_rule_conds.
+                  solve_q.
+                }
+              }
+              { destruct H.
+                { remember (edgeDownTo dtr oidx) as odown.
+                  destruct odown; auto.
+                  eapply eq_sym, edgeDownTo_Some in Heqodown; [|eassumption].
+                  dest; disc_rule_conds.
+                }
+                { destruct H as [rqUp [down [pidx ?]]]; dest.
+                  disc_rule_conds.
+                  rewrite rssQ_enqMsgs_rqs by assumption.
+                  solve_q.
+                }
+              }
+            }
+            { intro Hx.
+              elim (rqrsDTree_rsUp_down_not_eq Hsd _ _ H5 Hx).
+              reflexivity.
+            }
+
+      - (** case [RsBackRule] *)
+        good_footprint_get (obj_idx obj).
+        disc_rule_conds.
+        + (** case [FootprintReleasingUp] *)
+          destruct (eq_nat_dec cidx oidx); subst.
+          * find_if_inside.
+            { destruct H as [rqUp [down [pidx ?]]]; dest.
+              exists rqUp, down, pidx.
+              disc_rule_conds.
+
+              apply xor3_inv_3
+                with (C:= OLockedTo orqs (obj_idx obj) (rqi_midx_rsb rqi))
+                in H21; [dest|red; disc_rule_conds; eexists; intuition].
+
+              assert (length (findQ rqFrom (enqMP (rqi_midx_rsb rqi) rsm (deqMP (fst i) msgs))) = 0).
+              { solve_q; omega. }
+              rewrite H7; clear H7.
+
+              assert (length
+                        (rssQ (enqMP (rqi_midx_rsb rqi) rsm (deqMP (fst i) msgs))
+                              (rqi_midx_rsb rqi)) = 1).
+              { solve_q.
+                rewrite filter_app; simpl.
+                rewrite H8; simpl.
+                rewrite app_length; simpl.
+                unfold rssQ in H6, H19; omega.
+              }
+              rewrite H7; clear H7.
+
+              repeat split; try assumption; try omega.
+              { red; mred; simpl; mred. }
+              { xsnd; [discriminate|reflexivity|].
+                apply ONoLockTo_not_OLockedTo.
+                red in H20; red; mred.
+                simpl; mred; split; auto.
+              }
+            }
+            { destruct H; [left; assumption|right].
+              destruct H as [rqUp [down [pidx ?]]]; dest.
+              exfalso.
+              disc_rule_conds.
+              red in H20; mred.
+            }
+          * find_if_inside.
+            { apply upLockedInv_orqs_preserved_parent_none_up
+                with (orqs1:= orqs) (pidx:= obj_idx obj) (rqiu:= rqi);
+                auto; try (repeat (mred; simpl); fail).
+              { eapply upLockedInv_msgs_preserved; [eassumption| |].
+                { destruct H as [rqUp [down [pidx ?]]]; dest.
+                  disc_rule_conds.
+                  solve_q.
+                }
+                { destruct H as [rqUp [down [pidx ?]]]; dest.
+                  disc_rule_conds.
+                  solve_q.
+                }
+              }
+              { intro Hx.
+                elim (rqrsDTree_down_down_not_eq Hsd n H15 Hx).
+                reflexivity.
+              }
+            }
+            { apply upLockFreeInv_orqs_preserved_parent_none_up
+                with (orqs1:= orqs) (pidx:= obj_idx obj);
+                auto; try (repeat (mred; simpl); fail).
+              eapply upLockFreeInv_msgs_preserved; [eassumption| |].
+              { destruct H.
+                { remember (rqEdgeUpFrom dtr oidx) as orqUp.
+                  destruct orqUp; auto.
+                  eapply eq_sym, rqEdgeUpFrom_Some in HeqorqUp; [|eassumption].
+                  dest; disc_rule_conds.
+                }
+                { destruct H as [rqUp [down [pidx ?]]]; dest.
+                  disc_rule_conds.
+                  solve_q.
+                }
+              }
+              { destruct H.
+                { remember (edgeDownTo dtr oidx) as odown.
+                  destruct odown; auto.
+                  eapply eq_sym, edgeDownTo_Some in Heqodown; [|eassumption].
+                  dest; disc_rule_conds.
+                }
+                { destruct H as [rqUp [down [pidx ?]]]; dest.
+                  disc_rule_conds.
+                  solve_q.
+                }
+              }
+            }
+
+        + (** case [FootprintReleasingDown]-1 *)
+          destruct (eq_nat_dec (obj_idx upCObj) oidx); subst.
+          * find_if_inside.
+            { destruct H as [rqUp [down [pidx ?]]]; dest.
+              exists rqUp, down, pidx.
+              disc_rule_conds.
+
+              apply xor3_inv_3
+                with (C:= OLockedTo orqs (obj_idx obj) (rqi_midx_rsb rqi))
+                in H20; [dest|red; disc_rule_conds; eexists; intuition].
+
+              assert (length (findQ rqFrom (enqMP (rqi_midx_rsb rqi) rsm (deqMsgs (idsOf mins) msgs))) = 0).
+              { rewrite H18; solve_q.
+                omega.
+              }
+              rewrite H11; clear H11.
+
+              assert (length
+                        (rssQ (enqMP (rqi_midx_rsb rqi) rsm (deqMsgs (idsOf mins) msgs))
+                              (rqi_midx_rsb rqi)) = 1).
+              { rewrite H18; solve_q.
+                rewrite filter_app; simpl.
+                rewrite H8; simpl.
+                rewrite app_length; simpl.
+                unfold rssQ in H10, H17; omega.
+              }
+              rewrite H11; clear H11.
+
+              repeat split; try assumption; try omega.
+              { red; mred; simpl; mred.
+                destruct (porq@[upRq]); auto.
+              }
+              { xsnd; [discriminate|reflexivity|].
+                apply ONoLockTo_not_OLockedTo.
+                red in H19; red; mred.
+                simpl; split.
+                { mred.
+                  destruct (porq@[upRq]) as [rqiu|]; auto.
+                  destruct H19; auto.
+                }
+                { mred. }
+              }
+            }
+            { destruct H; [left; assumption|right].
+              destruct H as [rqUp [down [pidx ?]]]; dest.
+              exfalso.
+              disc_rule_conds.
+              red in H19; mred.
+            }
+          * find_if_inside.
+            { apply upLockedInv_orqs_preserved_parent_none_down
+                with (orqs1:= orqs) (pidx:= obj_idx obj) (rqiu:= rqi);
+                auto; try (repeat (mred; simpl); fail).
+              { eapply upLockedInv_msgs_preserved; [eassumption| |].
+                { destruct H as [rqUp [down [pidx ?]]]; dest.
+                  disc_rule_conds.
+                  rewrite H18; solve_q.
+                }
+                { destruct H as [rqUp [down [pidx ?]]]; dest.
+                  disc_rule_conds.
+                  rewrite H18; solve_q.
+                }
+              }
+              { intro Hx.
+                elim (rqrsDTree_down_down_not_eq Hsd n H11 Hx).
+                reflexivity.
+              }
+            }
+            { apply upLockFreeInv_orqs_preserved_parent_none_down
+                with (orqs1:= orqs) (pidx:= obj_idx obj);
+                auto; try (repeat (mred; simpl); fail).
+              eapply upLockFreeInv_msgs_preserved; [eassumption| |].
+              { destruct H.
+                { remember (rqEdgeUpFrom dtr oidx) as orqUp.
+                  destruct orqUp; auto.
+                  eapply eq_sym, rqEdgeUpFrom_Some in HeqorqUp; [|eassumption].
+                  dest; disc_rule_conds.
+                }
+                { destruct H as [rqUp [down [pidx ?]]]; dest.
+                  disc_rule_conds.
+                  rewrite H18; solve_q.
+                }
+              }
+              { destruct H.
+                { remember (edgeDownTo dtr oidx) as odown.
+                  destruct odown; auto.
+                  eapply eq_sym, edgeDownTo_Some in Heqodown; [|eassumption].
+                  dest; disc_rule_conds.
+                }
+                { destruct H as [rqUp [down [pidx ?]]]; dest.
+                  disc_rule_conds.
+                  rewrite H18; solve_q.
+                }
+              }
+            }
+
+        + (** case [FootprintReleasingDown]-2 *)
+          find_if_inside.
+          * apply upLockedInv_orqs_preserved_parent_none_down
+              with (orqs1:= orqs) (pidx:= obj_idx obj) (rqiu:= rqi);
+              auto; try (repeat (mred; simpl); fail).
+            { eapply upLockedInv_msgs_preserved; [eassumption| |].
+              { destruct H as [rqUp [down [pidx ?]]]; dest.
+                disc_rule_conds.
+                rewrite H18; solve_q.
+              }
+              { destruct H as [rqUp [down [pidx ?]]]; dest.
+                disc_rule_conds.
+                rewrite H18; solve_q.
+              }
+            }
+            { intro Hx.
+              elim (rqrsDTree_rsUp_down_not_eq Hsd _ _ H6 Hx).
+              reflexivity.
+            }
+          * apply upLockFreeInv_orqs_preserved_parent_none_down
+              with (orqs1:= orqs) (pidx:= obj_idx obj);
+              auto; try (repeat (mred; simpl); fail).
+            eapply upLockFreeInv_msgs_preserved; [eassumption| |].
+            { destruct H.
+              { remember (rqEdgeUpFrom dtr oidx) as orqUp.
+                destruct orqUp; auto.
+                eapply eq_sym, rqEdgeUpFrom_Some in HeqorqUp; [|eassumption].
+                dest; disc_rule_conds.
+              }
+              { destruct H as [rqUp [down [pidx ?]]]; dest.
+                disc_rule_conds.
+                rewrite H18; solve_q.
+              }
+            }
+            { destruct H.
+              { remember (edgeDownTo dtr oidx) as odown.
+                destruct odown; auto.
+                eapply eq_sym, edgeDownTo_Some in Heqodown; [|eassumption].
+                dest; disc_rule_conds.
+              }
+              { destruct H as [rqUp [down [pidx ?]]]; dest.
+                disc_rule_conds.
+                rewrite H18; solve_q.
+              }
+            }
+
+      - (** case [RsDownRqDownRule] *)
+        find_if_inside.
+        + disc_rule_conds.
+          eapply upLockedInv_orqs_preserved_rs_rq
+            with (orqs1:= orqs) (pidx:= obj_idx obj) (rqiu:= rqi1) (rqid:= rqi0);
+            auto; try (repeat (mred; simpl); fail).
+          eapply upLockedInv_msgs_preserved; [eassumption| |].
+          * destruct H as [rqUp [down [pidx ?]]]; dest.
+            disc_rule_conds.
+            solve_q.
+          * destruct H as [rqUp [down [pidx ?]]]; dest.
+            disc_rule_conds.
+            rewrite rssQ_enqMsgs_rqs by assumption.
+            solve_q.
+        + disc_rule_conds.
+          eapply upLockFreeInv_orqs_preserved_rs_rq
+            with (orqs1:= orqs) (pidx:= obj_idx obj) (rqiu:= rqi1) (rqid:= rqi0);
+            auto; try (repeat (mred; simpl); fail).
+          eapply upLockFreeInv_msgs_preserved; [eassumption| |].
+          * destruct H.
+            { remember (rqEdgeUpFrom dtr oidx) as orqUp.
+              destruct orqUp; auto.
+              eapply eq_sym, rqEdgeUpFrom_Some in HeqorqUp; [|eassumption].
+              dest; disc_rule_conds.
+            }
+            { destruct H as [rqUp [down [pidx ?]]]; dest.
+              disc_rule_conds.
+              solve_q.
+            }
+          * destruct H.
+            { remember (edgeDownTo dtr oidx) as odown.
+              destruct odown; auto.
+              eapply eq_sym, edgeDownTo_Some in Heqodown; [|eassumption].
+              dest; disc_rule_conds.
+            }
+            { destruct H as [rqUp [down [pidx ?]]]; dest.
+              disc_rule_conds.
+              rewrite rssQ_enqMsgs_rqs by assumption.
+              solve_q.
+            }
+    Qed.
+
+    Lemma upLockInvORq_step_int_other:
+      forall oidx orq,
+        UpLockInvORq orqs msgs oidx orq ->
+        In oidx (map (@obj_idx _) (sys_objs sys)) ->
+        GoodRqRsRule dtr sys (obj_idx obj) rule ->
+        obj_idx obj <> oidx ->
+        parentIdxOf dtr oidx <> Some (obj_idx obj) ->
+        UpLockInvORq (orqs+[obj_idx obj <- norq])
+                     (enqMsgs mouts (deqMsgs (idsOf mins) msgs)) oidx
+                     orq.
+    Proof.
+      intros.
+      destruct Hsd.
+      red in H; red.
+      good_rqrs_rule_cases rule.
+
+      - (** case [ImmDownRule] *)
+        find_if_inside.
+        + apply upLockedInv_orqs_preserved_non_parent_update; auto.
+          apply upLockedInv_msgs_preserved with (msgs1:= msgs);
+            [assumption| |].
+          * destruct H as [rqUp [down [pidx ?]]]; dest.
+            disc_rule_conds.
+            solve_q.
+          * destruct H as [rqUp [down [pidx ?]]]; dest.
+            disc_rule_conds.
+            solve_q.
+        + apply upLockFreeInv_orqs_preserved_non_parent_update; auto.
+          apply upLockFreeInv_msgs_preserved with (msgs1:= msgs);
+            [assumption| |].
+          * destruct H.
+            { remember (rqEdgeUpFrom dtr oidx) as orqUp.
+              destruct orqUp; auto.
+              eapply eq_sym, rqEdgeUpFrom_Some in HeqorqUp; [|eassumption].
+              dest; disc_rule_conds.
+            }
+            { destruct H as [rqUp [down [pidx ?]]]; dest.
+              disc_rule_conds.
+              solve_q.
+            }
+          * destruct H.
+            { remember (edgeDownTo dtr oidx) as odown.
+              destruct odown; auto.
+              eapply eq_sym, edgeDownTo_Some in Heqodown; [|eassumption].
+              dest; disc_rule_conds.
+            }
+            { destruct H as [rqUp [down [pidx ?]]]; dest.
+              disc_rule_conds.
+              solve_q.
+            }
+
+      - (** case [ImmUpRule] *)
+        find_if_inside.
+        + apply upLockedInv_orqs_preserved_non_parent_update; auto.
+          apply upLockedInv_msgs_preserved with (msgs1:= msgs);
+            [assumption| |].
+          * destruct H as [rqUp [down [pidx ?]]]; dest.
+            disc_rule_conds.
+            solve_q.
+          * destruct H as [rqUp [down [pidx ?]]]; dest.
+            disc_rule_conds.
+            solve_q.
+        + apply upLockFreeInv_orqs_preserved_non_parent_update; auto.
+          apply upLockFreeInv_msgs_preserved with (msgs1:= msgs);
+            [assumption| |].
+          * destruct H.
+            { remember (rqEdgeUpFrom dtr oidx) as orqUp.
+              destruct orqUp; auto.
+              eapply eq_sym, rqEdgeUpFrom_Some in HeqorqUp; [|eassumption].
+              dest; disc_rule_conds.
+            }
+            { destruct H as [rqUp [down [pidx ?]]]; dest.
+              disc_rule_conds.
+              solve_q.
+            }
+          * destruct H.
+            { remember (edgeDownTo dtr oidx) as odown.
+              destruct odown; auto.
+              eapply eq_sym, edgeDownTo_Some in Heqodown; [|eassumption].
+              dest; disc_rule_conds.
+            }
+            { destruct H as [rqUp [down [pidx ?]]]; dest.
+              disc_rule_conds.
+              solve_q.
+            }
+        
+      - (** case [RqFwdRule] *)
+        disc_rule_conds.
+
+        + find_if_inside.
+          * apply upLockedInv_orqs_preserved_non_parent_update; auto.
+            apply upLockedInv_msgs_preserved with (msgs1:= msgs);
+              [assumption| |].
+            { destruct H as [rqUp [down [pidx ?]]]; dest.
+              disc_rule_conds.
+              solve_q.
+            }
+            { destruct H as [rqUp [down [pidx ?]]]; dest.
+              disc_rule_conds.
+              solve_q.
+            }
+          * apply upLockFreeInv_orqs_preserved_non_parent_update; auto.
+            apply upLockFreeInv_msgs_preserved with (msgs1:= msgs);
+              [assumption| |].
+            { destruct H.
+              { remember (rqEdgeUpFrom dtr oidx) as orqUp.
+                destruct orqUp; auto.
+                eapply eq_sym, rqEdgeUpFrom_Some in HeqorqUp; [|eassumption].
+                dest; disc_rule_conds.
+              }
+              { destruct H as [rqUp [down [pidx ?]]]; dest.
+                disc_rule_conds.
+                solve_q.
+              }
+            }
+            { destruct H.
+              { remember (edgeDownTo dtr oidx) as odown.
+                destruct odown; auto.
+                eapply eq_sym, edgeDownTo_Some in Heqodown; [|eassumption].
+                dest; disc_rule_conds.
+              }
+              { destruct H as [rqUp [down [pidx ?]]]; dest.
+                disc_rule_conds.
+                solve_q.
+              }
+            }
+
+        + find_if_inside.
+          * apply upLockedInv_orqs_preserved_non_parent_update; auto.
+            apply upLockedInv_msgs_preserved with (msgs1:= msgs);
+              [assumption| |].
+            { destruct H as [rqUp [down [pidx ?]]]; dest.
+              disc_rule_conds.
+              solve_q.
+            }
+            { destruct H as [rqUp [down [pidx ?]]]; dest.
+              disc_rule_conds.
+              solve_q.
+            }
+          * apply upLockFreeInv_orqs_preserved_non_parent_update; auto.
+            apply upLockFreeInv_msgs_preserved with (msgs1:= msgs);
+              [assumption| |].
+            { destruct H.
+              { remember (rqEdgeUpFrom dtr oidx) as orqUp.
+                destruct orqUp; auto.
+                eapply eq_sym, rqEdgeUpFrom_Some in HeqorqUp; [|eassumption].
+                dest; disc_rule_conds.
+              }
+              { destruct H as [rqUp [down [pidx ?]]]; dest.
+                disc_rule_conds.
+                solve_q.
+              }
+            }
+            { destruct H.
+              { remember (edgeDownTo dtr oidx) as odown.
+                destruct odown; auto.
+                eapply eq_sym, edgeDownTo_Some in Heqodown; [|eassumption].
+                dest; disc_rule_conds.
+              }
+              { destruct H as [rqUp [down [pidx ?]]]; dest.
+                disc_rule_conds.
+                solve_q.
+              }
+            }
+
+        + find_if_inside.
+          * apply upLockedInv_orqs_preserved_non_parent_update; auto.
+            apply upLockedInv_msgs_preserved with (msgs1:= msgs);
+              [assumption| |].
+            { destruct H as [rqUp [down [pidx ?]]]; dest.
+              disc_rule_conds.
+              solve_q.
+            }
+            { destruct H as [rqUp [down [pidx ?]]]; dest.
+              disc_rule_conds.
+              solve_q.
+            }
+          * apply upLockFreeInv_orqs_preserved_non_parent_update; auto.
+            apply upLockFreeInv_msgs_preserved with (msgs1:= msgs);
+              [assumption| |].
+            { destruct H.
+              { remember (rqEdgeUpFrom dtr oidx) as orqUp.
+                destruct orqUp; auto.
+                eapply eq_sym, rqEdgeUpFrom_Some in HeqorqUp; [|eassumption].
+                dest; disc_rule_conds.
+              }
+              { destruct H as [rqUp [down [pidx ?]]]; dest.
+                disc_rule_conds.
+                solve_q.
+              }
+            }
+            { destruct H.
+              { remember (edgeDownTo dtr oidx) as odown.
+                destruct odown; auto.
+                eapply eq_sym, edgeDownTo_Some in Heqodown; [|eassumption].
+                dest; disc_rule_conds.
+              }
+              { destruct H as [rqUp [down [pidx ?]]]; dest.
+                disc_rule_conds.
+                solve_q.
+              }
+            }
+
+      - (** case [RsBackRule] *)
+        good_footprint_get (obj_idx obj).
+        disc_rule_conds.
+
+        + find_if_inside.
+          * apply upLockedInv_orqs_preserved_non_parent_update; auto.
+            apply upLockedInv_msgs_preserved with (msgs1:= msgs);
+              [assumption| |].
+            { destruct H as [rqUp [down [pidx ?]]]; dest.
+              disc_rule_conds.
+              solve_q.
+            }
+            { destruct H as [rqUp [down [pidx ?]]]; dest.
+              disc_rule_conds.
+              solve_q.
+            }
+          * apply upLockFreeInv_orqs_preserved_non_parent_update; auto.
+            apply upLockFreeInv_msgs_preserved with (msgs1:= msgs);
+              [assumption| |].
+            { destruct H.
+              { remember (rqEdgeUpFrom dtr oidx) as orqUp.
+                destruct orqUp; auto.
+                eapply eq_sym, rqEdgeUpFrom_Some in HeqorqUp; [|eassumption].
+                dest; disc_rule_conds.
+              }
+              { destruct H as [rqUp [down [pidx ?]]]; dest.
+                disc_rule_conds.
+                solve_q.
+              }
+            }
+            { destruct H.
+              { remember (edgeDownTo dtr oidx) as odown.
+                destruct odown; auto.
+                eapply eq_sym, edgeDownTo_Some in Heqodown; [|eassumption].
+                dest; disc_rule_conds.
+              }
+              { destruct H as [rqUp [down [pidx ?]]]; dest.
+                disc_rule_conds.
+                solve_q.
+              }
+            }
+
+        + rewrite <-H19 in H13.
+          find_if_inside.
+          * apply upLockedInv_orqs_preserved_non_parent_update; auto.
+            apply upLockedInv_msgs_preserved with (msgs1:= msgs);
+              [assumption| |].
+            { destruct H as [rqUp [down [pidx ?]]]; dest.
+              disc_rule_conds.
+              solve_q.
+            }
+            { destruct H as [rqUp [down [pidx ?]]]; dest.
+              disc_rule_conds.
+              solve_q.
+            }
+          * apply upLockFreeInv_orqs_preserved_non_parent_update; auto.
+            apply upLockFreeInv_msgs_preserved with (msgs1:= msgs);
+              [assumption| |].
+            { destruct H.
+              { remember (rqEdgeUpFrom dtr oidx) as orqUp.
+                destruct orqUp; auto.
+                eapply eq_sym, rqEdgeUpFrom_Some in HeqorqUp; [|eassumption].
+                dest; disc_rule_conds.
+              }
+              { destruct H as [rqUp [down [pidx ?]]]; dest.
+                disc_rule_conds.
+                solve_q.
+              }
+            }
+            { destruct H.
+              { remember (edgeDownTo dtr oidx) as odown.
+                destruct odown; auto.
+                eapply eq_sym, edgeDownTo_Some in Heqodown; [|eassumption].
+                dest; disc_rule_conds.
+              }
+              { destruct H as [rqUp [down [pidx ?]]]; dest.
+                disc_rule_conds.
+                solve_q.
+              }
+            }
+
+        + rewrite <-H19 in H8.
+          find_if_inside.
+          * apply upLockedInv_orqs_preserved_non_parent_update; auto.
+            apply upLockedInv_msgs_preserved with (msgs1:= msgs);
+              [assumption| |].
+            { destruct H as [rqUp [down [pidx ?]]]; dest.
+              disc_rule_conds.
+              solve_q.
+            }
+            { destruct H as [rqUp [down [pidx ?]]]; dest.
+              disc_rule_conds.
+              solve_q.
+            }
+          * apply upLockFreeInv_orqs_preserved_non_parent_update; auto.
+            apply upLockFreeInv_msgs_preserved with (msgs1:= msgs);
+              [assumption| |].
+            { destruct H.
+              { remember (rqEdgeUpFrom dtr oidx) as orqUp.
+                destruct orqUp; auto.
+                eapply eq_sym, rqEdgeUpFrom_Some in HeqorqUp; [|eassumption].
+                dest; disc_rule_conds.
+              }
+              { destruct H as [rqUp [down [pidx ?]]]; dest.
+                disc_rule_conds.
+                solve_q.
+              }
+            }
+            { destruct H.
+              { remember (edgeDownTo dtr oidx) as odown.
+                destruct odown; auto.
+                eapply eq_sym, edgeDownTo_Some in Heqodown; [|eassumption].
+                dest; disc_rule_conds.
+              }
+              { destruct H as [rqUp [down [pidx ?]]]; dest.
+                disc_rule_conds.
+                solve_q.
+              }
+            }
+
+      - (** case [RsDownRqDownRule] *)
+        disc_rule_conds.
+        find_if_inside.
+        + apply upLockedInv_orqs_preserved_non_parent_update; auto.
+          apply upLockedInv_msgs_preserved with (msgs1:= msgs);
+            [assumption| |].
+          * destruct H as [rqUp [down [pidx ?]]]; dest.
+            disc_rule_conds.
+            solve_q.
+          * destruct H as [rqUp [down [pidx ?]]]; dest.
+            disc_rule_conds.
+            solve_q.
+        + apply upLockFreeInv_orqs_preserved_non_parent_update; auto.
+          apply upLockFreeInv_msgs_preserved with (msgs1:= msgs);
+            [assumption| |].
+          * destruct H.
+            { remember (rqEdgeUpFrom dtr oidx) as orqUp.
+              destruct orqUp; auto.
+              eapply eq_sym, rqEdgeUpFrom_Some in HeqorqUp; [|eassumption].
+              dest; disc_rule_conds.
+            }
+            { destruct H as [rqUp [down [pidx ?]]]; dest.
+              disc_rule_conds.
+              solve_q.
+            }
+          * destruct H.
+            { remember (edgeDownTo dtr oidx) as odown.
+              destruct odown; auto.
+              eapply eq_sym, edgeDownTo_Some in Heqodown; [|eassumption].
+              dest; disc_rule_conds.
+            }
+            { destruct H as [rqUp [down [pidx ?]]]; dest.
+              disc_rule_conds.
+              solve_q.
+            }
+    Qed.
+    
+    Lemma upLockInv_step_int:
+      UpLockInv {| bst_oss := oss; bst_orqs := orqs; bst_msgs := msgs |} ->
+      UpLockInv {| bst_oss := (oss) +[ obj_idx obj <- nost];
+                   bst_orqs := (orqs) +[ obj_idx obj <- norq];
+                   bst_msgs := enqMsgs mouts (deqMsgs (idsOf mins) msgs) |}.
+    Proof.
+      intros.
+      do 2 red; simpl; intros.
+      good_rqrs_rule_get rule.
+      specialize (H _ H0); simpl in H; dest.
+
+      M.cmp (obj_idx obj) oidx; mred; simpl in *.
+      - (** case [oidx = obj_idx obj] *)
+        apply upLockInvORq_step_int_me; assumption.
+      - (** case [oidx <> obj_idx obj] *)
+        remember (parentIdxOf dtr oidx) as opidx.
+        destruct opidx as [pidx|].
+        + destruct (eq_nat_dec (obj_idx obj) pidx); subst.
+          * apply upLockInvORq_step_int_parent; auto.
+          * apply upLockInvORq_step_int_other; auto.
+            rewrite <-Heqopidx.
+            intro Hx; elim n0; inv Hx; reflexivity.
+        + apply upLockInvORq_step_int_other; auto.
+          rewrite <-Heqopidx; discriminate.
+    Qed.
+
+  End InternalStep.
+
+  Lemma upLockInv_step:
+    InvStep sys step_m UpLockInv.
+  Proof.
+    red; intros.
+    inv H1.
+    - auto.
+    - apply upLockInv_step_ext_in; auto.
+    - apply upLockInv_step_ext_out; auto.
+    - eapply upLockInv_step_int; eauto.
+      eapply footprints_ok; eassumption.
+  Qed.
+
+  Lemma upLockInv_ok:
+    InvReachable sys step_m UpLockInv.
+  Proof.
+    apply inv_reachable.
+    - apply upLockInv_init.
+    - apply upLockInv_step.
+  Qed.
+  
+End UpLockInv.
+
+Close Scope list.
+Close Scope fmap.
+
